<?xml version="1.0"?>


<!DOCTYPE rdf:RDF [
    <!ENTITY owl "http://www.w3.org/2002/07/owl#" >
    <!ENTITY swrl "http://www.w3.org/2003/11/swrl#" >
    <!ENTITY dc "http://purl.org/dc/elements/1.1/" >
    <!ENTITY swrlb "http://www.w3.org/2003/11/swrlb#" >
    <!ENTITY xsd "http://www.w3.org/2001/XMLSchema#" >
    <!ENTITY rdfs "http://www.w3.org/2000/01/rdf-schema#" >
    <!ENTITY rdf "http://www.w3.org/1999/02/22-rdf-syntax-ns#" >
]>


<rdf:RDF xmlns="http://purl.org/ceu/lco#"
     xml:base="http://purl.org/ceu/lco"
     xmlns:rdf="http://www.w3.org/1999/02/22-rdf-syntax-ns#"
     xmlns:owl="http://www.w3.org/2002/07/owl#"
     xmlns:swrlb="http://www.w3.org/2003/11/swrlb#"
     xmlns:swrl="http://www.w3.org/2003/11/swrl#"
     xmlns:xsd="http://www.w3.org/2001/XMLSchema#"
     xmlns:rdfs="http://www.w3.org/2000/01/rdf-schema#"
     xmlns:dc="http://purl.org/dc/elements/1.1/">
    <owl:Ontology rdf:about="http://purl.org/ceu/simeon">
        <rdfs:label xml:lang="en">SIMEON Ontology</rdfs:label>
        <rdfs:label xml:lang="es">Ontología SIMEON</rdfs:label>
        <dc:license xml:lang="en">Attribution-ShareAlike 4.0 International Creative Commons license (http://creativecommons.org/licenses/by-sa/4.0/)</dc:license>
        <rdfs:comment xml:lang="en">SIMEON ontology allow to establish similarity measures between ontology objets and collections.</rdfs:comment>
        <dc:abstract xml:lang="en">SIMEON ontology allow to establish similarity measures between ontology objets and collections.</dc:abstract>
        <owl:versionInfo xml:lang="en">Version 1.0 2015/07/01</owl:versionInfo>
        <dc:creator xml:lang="es">Alfredo Sánchez Alberca (asalber@ceu.es) &lt;http://aprendeconalf.es/foaf.rdf&gt;</dc:creator>
        <rdfs:comment xml:lang="es">La ontología SIMEON permite establecer medidas de similitud entre los objetos y colecciones de objetos de las ontologías.</rdfs:comment>
        <dc:abstract xml:lang="es">La ontología SIMEON permite establecer medidas de similitud entre los objetos y colecciones de objetos de las ontologías.</dc:abstract>
        <dc:license xml:lang="es">Licencia de Creative Commons Reconocimiento-CompartirIgual 4.0 Internacional (http://creativecommons.org/licenses/by-sa/4.0/).</dc:license>
        <owl:versionInfo xml:lang="es">Versión 1.0 01/07/2015</owl:versionInfo>
        <owl:versionIRI rdf:resource="http://purl.org/ceu/simeon/1.0"/>
    </owl:Ontology>
    


    <!-- 
    ///////////////////////////////////////////////////////////////////////////////////////
    //
    // Object Properties
    //
    ///////////////////////////////////////////////////////////////////////////////////////
     -->

    


    <!-- http://purl.org/ceu/simeon#comparesObject -->

    <owl:ObjectProperty rdf:about="http://purl.org/ceu/simeon#comparesObject">
        <rdfs:label xml:lang="en">compares object</rdfs:label>
        <rdfs:label xml:lang="es">compara objeto</rdfs:label>
        <rdfs:comment xml:lang="en">Property that relates a comparison method with an individual that is compared with that method.</rdfs:comment>
        <rdfs:comment xml:lang="es">Propiedad que relaciona un método de comparación con un individuo que es comparado mediante ese método.</rdfs:comment>
        <rdfs:domain rdf:resource="http://purl.org/ceu/simeon#ComparisonMethod"/>
        <rdfs:range rdf:resource="&owl;Thing"/>
        <owl:propertyChainAxiom rdf:parseType="Collection">
            <rdf:Description rdf:about="http://purl.org/ceu/simeon#usedByComparisonMeasure"/>
            <rdf:Description rdf:about="http://purl.org/ceu/simeon#hasTargetObject"/>
        </owl:propertyChainAxiom>
        <owl:propertyChainAxiom rdf:parseType="Collection">
            <rdf:Description rdf:about="http://purl.org/ceu/simeon#usedByComparisonMeasure"/>
            <rdf:Description rdf:about="http://purl.org/ceu/simeon#hasSourceObject"/>
        </owl:propertyChainAxiom>
    </owl:ObjectProperty>
    


    <!-- http://purl.org/ceu/simeon#hasAlgorithm -->

    <owl:ObjectProperty rdf:about="http://purl.org/ceu/simeon#hasAlgorithm">
        <rdfs:label xml:lang="en">has algorithm</rdfs:label>
        <rdfs:label xml:lang="es">tiene algoritmo</rdfs:label>
        <rdfs:comment xml:lang="en">Property that relates a comparison method with the algorithm or calculation procedure that uses.</rdfs:comment>
        <rdfs:comment xml:lang="es">Propiedad que relaciona un método de comparación con el algoritmo o procedimiento de cálculo que utiliza.</rdfs:comment>
        <rdfs:range rdf:resource="http://purl.org/ceu/simeon#Algorithm"/>
        <rdfs:domain rdf:resource="http://purl.org/ceu/simeon#ComparisonMethod"/>
    </owl:ObjectProperty>
    


    <!-- http://purl.org/ceu/simeon#hasDomain -->

    <owl:ObjectProperty rdf:about="http://purl.org/ceu/simeon#hasDomain">
        <rdfs:label xml:lang="en">has domain</rdfs:label>
        <rdfs:label xml:lang="es">tiene dominio</rdfs:label>
        <rdfs:comment xml:lang="en">Property that relates a comparison method with the types of objects or entities that compares.</rdfs:comment>
        <rdfs:comment xml:lang="es">Propiedad que relaciona un método de comparación con el tipo de objetos o entidades que compara.</rdfs:comment>
        <rdfs:domain rdf:resource="http://purl.org/ceu/simeon#ComparisonMethod"/>
    </owl:ObjectProperty>
    


    <!-- http://purl.org/ceu/simeon#hasReference -->

    <owl:ObjectProperty rdf:about="http://purl.org/ceu/simeon#hasReference">
        <rdfs:label xml:lang="en">has reference</rdfs:label>
        <rdfs:label xml:lang="es">tiene referencia</rdfs:label>
        <rdfs:comment xml:lang="en">Property that relates a comparison method with a bibliographic reference where the method is explained.</rdfs:comment>
        <rdfs:comment xml:lang="es">Propiedad que relaciona un método de comparación con una referencia bibliográfica donde se describe el método.</rdfs:comment>
        <rdfs:domain rdf:resource="http://purl.org/ceu/simeon#ComparisonMethod"/>
        <rdfs:range rdf:resource="http://purl.org/dc/terms/BibliographicResource"/>
    </owl:ObjectProperty>
    


    <!-- http://purl.org/ceu/simeon#hasSourceObject -->

    <owl:ObjectProperty rdf:about="http://purl.org/ceu/simeon#hasSourceObject">
        <rdf:type rdf:resource="&owl;FunctionalProperty"/>
        <rdfs:label xml:lang="en">has source object</rdfs:label>
        <rdfs:label xml:lang="es">tiene objeto origen</rdfs:label>
        <rdfs:comment xml:lang="en">A similarity measurement expresses the similarity degree of a source object with a target object. This property that relates a similarity measure with the source object.</rdfs:comment>
        <rdfs:comment xml:lang="es">Una medida de similitud establece el grado de parecido de un objeto origen con otro destino. Esta propiedad relaciona la medida de similitud con el objeto origen.</rdfs:comment>
        <rdfs:domain rdf:resource="http://purl.org/ceu/simeon#ObjectComparisonMeasure"/>
        <rdfs:range rdf:resource="&owl;Thing"/>
    </owl:ObjectProperty>
    


    <!-- http://purl.org/ceu/simeon#hasTargetObject -->

    <owl:ObjectProperty rdf:about="http://purl.org/ceu/simeon#hasTargetObject">
        <rdf:type rdf:resource="&owl;FunctionalProperty"/>
        <rdfs:label xml:lang="en">has target object</rdfs:label>
        <rdfs:label xml:lang="es">tiene objeto destino</rdfs:label>
        <rdfs:comment xml:lang="en">A similarity measurement expresses the similarity degree of a source object with a target object. This property that relates a similarity measure with the target object.</rdfs:comment>
        <rdfs:comment xml:lang="es">Una medida de similitud establece el grado de parecido de un objeto origen con otro destino. Esta propiedad relaciona la medida de similitud con el objeto destino cuando se trata de un literal.</rdfs:comment>
        <rdfs:comment xml:lang="es">Una medida de similitud establece el grado de parecido de un objeto origen con otro destino. Esta propiedad relaciona la medida de similitud con el objeto destino.</rdfs:comment>
        <rdfs:domain rdf:resource="http://purl.org/ceu/simeon#ObjectComparisonMeasure"/>
        <rdfs:range rdf:resource="&owl;Thing"/>
    </owl:ObjectProperty>
    


    <!-- http://purl.org/ceu/simeon#isPerformedBy -->

    <owl:ObjectProperty rdf:about="http://purl.org/ceu/simeon#isPerformedBy">
        <rdf:type rdf:resource="&owl;FunctionalProperty"/>
        <rdfs:label xml:lang="en">is performed by</rdfs:label>
        <rdfs:label xml:lang="es">es realizada por</rdfs:label>
        <rdfs:comment xml:lang="en">Property that relates a subjective comparison measure with the person that performs that measure.</rdfs:comment>
        <rdfs:comment xml:lang="es">Propiedad que relaciona una medida de comparación subjetiva con la persona que realiza esa medida.</rdfs:comment>
        <rdfs:domain rdf:resource="http://purl.org/ceu/simeon#ComparisonMeasure"/>
        <rdfs:range rdf:resource="http://purl.org/dc/terms/Agent"/>
    </owl:ObjectProperty>
    


    <!-- http://purl.org/ceu/simeon#usedByComparisonMeasure -->

    <owl:ObjectProperty rdf:about="http://purl.org/ceu/simeon#usedByComparisonMeasure">
        <rdf:type rdf:resource="&owl;InverseFunctionalProperty"/>
        <rdfs:label xml:lang="en">used by comparsion measure</rdfs:label>
        <rdfs:label xml:lang="es">usada por medida de comapración</rdfs:label>
        <rdfs:comment xml:lang="en">Property that relates a comparison method with a comparison measure calculated with that method.</rdfs:comment>
        <rdfs:comment xml:lang="es">Propieda que relaciona un método de comparación con una medida de comparación calculada con ese método.</rdfs:comment>
        <rdfs:range rdf:resource="http://purl.org/ceu/simeon#ComparisonMeasure"/>
        <rdfs:domain rdf:resource="http://purl.org/ceu/simeon#ComparisonMethod"/>
    </owl:ObjectProperty>
    


    <!-- http://purl.org/ceu/simeon#usesComparisonMethod -->

    <owl:ObjectProperty rdf:about="http://purl.org/ceu/simeon#usesComparisonMethod">
        <rdf:type rdf:resource="&owl;FunctionalProperty"/>
        <rdfs:label xml:lang="en">uses comparison method</rdfs:label>
        <rdfs:label xml:lang="es">usa método de comparación</rdfs:label>
        <rdfs:comment xml:lang="en">Property that relates a comparison measure with the comparison method used to get it.</rdfs:comment>
        <rdfs:comment xml:lang="es">Propiedad que relaciona una medida de comparación con el método de comparación utilizado para obtenerla.</rdfs:comment>
        <rdfs:domain rdf:resource="http://purl.org/ceu/simeon#ComparisonMeasure"/>
        <rdfs:range rdf:resource="http://purl.org/ceu/simeon#ComparisonMethod"/>
        <owl:inverseOf rdf:resource="http://purl.org/ceu/simeon#usedByComparisonMeasure"/>
    </owl:ObjectProperty>
    


    <!-- 
    ///////////////////////////////////////////////////////////////////////////////////////
    //
    // Data properties
    //
    ///////////////////////////////////////////////////////////////////////////////////////
     -->

    


    <!-- http://purl.org/ceu/simeon#hasSourceData -->

    <owl:DatatypeProperty rdf:about="http://purl.org/ceu/simeon#hasSourceData">
        <rdf:type rdf:resource="&owl;FunctionalProperty"/>
        <rdfs:label xml:lang="en">has source data</rdfs:label>
        <rdfs:label xml:lang="es">tiene dato origen</rdfs:label>
        <rdfs:comment xml:lang="en">A similarity measurement expresses the similarity degree of a source object with a target object. This property that relates a similarity measure with the source object when that object is a literal.</rdfs:comment>
        <rdfs:comment xml:lang="es">Una medida de similitud establece el grado de parecido de un objeto origen con otro destino. Esta propiedad relaciona la medida de similitud con el objeto origen cuando se trata de un literal.</rdfs:comment>
        <rdfs:domain rdf:resource="http://purl.org/ceu/simeon#DataComparisonMeasure"/>
        <rdfs:range rdf:resource="&rdfs;Literal"/>
    </owl:DatatypeProperty>
    


    <!-- http://purl.org/ceu/simeon#hasTargetData -->

    <owl:DatatypeProperty rdf:about="http://purl.org/ceu/simeon#hasTargetData">
        <rdf:type rdf:resource="&owl;FunctionalProperty"/>
        <rdfs:label xml:lang="en">has target data</rdfs:label>
        <rdfs:label xml:lang="es">tiene dato destino</rdfs:label>
        <rdfs:comment xml:lang="en">A similarity measurement expresses the similarity degree of a source object with a target object. This property that relates a similarity measure with the target object when that object is a literal.</rdfs:comment>
        <rdfs:comment xml:lang="es">Una medida de similitud establece el grado de parecido de un objeto origen con otro destino. Esta propiedad relaciona la medida de similitud con el objeto destino cuando se trata de un literal.</rdfs:comment>
        <rdfs:domain rdf:resource="http://purl.org/ceu/simeon#DataComparisonMeasure"/>
        <rdfs:range rdf:resource="&rdfs;Literal"/>
    </owl:DatatypeProperty>
    


    <!-- http://purl.org/ceu/simeon#hasValue -->

    <owl:DatatypeProperty rdf:about="http://purl.org/ceu/simeon#hasValue">
        <rdf:type rdf:resource="&owl;FunctionalProperty"/>
        <rdfs:label xml:lang="en">has value</rdfs:label>
        <rdfs:label xml:lang="es">tiene valor</rdfs:label>
        <rdfs:comment xml:lang="en">Property that relates a similiarity measure with the value of the measure.</rdfs:comment>
        <rdfs:comment xml:lang="es">Propiedad que relaciona una medida de similitud con el valor de la medida.</rdfs:comment>
        <rdfs:domain rdf:resource="http://purl.org/ceu/simeon#ComparisonMeasure"/>
        <rdfs:range>
            <rdfs:Datatype>
                <owl:onDatatype rdf:resource="&xsd;decimal"/>
                <owl:withRestrictions rdf:parseType="Collection">
                    <rdf:Description>
                        <xsd:minInclusive rdf:datatype="&xsd;decimal">0.0</xsd:minInclusive>
                    </rdf:Description>
                </owl:withRestrictions>
            </rdfs:Datatype>
        </rdfs:range>
    </owl:DatatypeProperty>
    


    <!-- 
    ///////////////////////////////////////////////////////////////////////////////////////
    //
    // Classes
    //
    ///////////////////////////////////////////////////////////////////////////////////////
     -->

    


    <!-- http://purl.obolibrary.org/obo/IAO_0000064 -->

    <owl:Class rdf:about="http://purl.obolibrary.org/obo/IAO_0000064">
        <rdfs:label xml:lang="en">Algorithm</rdfs:label>
        <rdfs:label xml:lang="es">Algoritmo</rdfs:label>
        <owl:equivalentClass rdf:resource="http://purl.org/ceu/simeon#Algorithm"/>
        <rdfs:comment xml:lang="en">An algorithm is a procedure for doing some calculations.</rdfs:comment>
        <rdfs:seeAlso xml:lang="en">The software ontology: http://theswo.sourceforge.net/</rdfs:seeAlso>
        <rdfs:seeAlso xml:lang="es">La ontología de software: http://theswo.sourceforge.net/</rdfs:seeAlso>
        <rdfs:comment xml:lang="es">Un algoritmo es un procedimiento para realizar unos cálculos.</rdfs:comment>
    </owl:Class>
    


    <!-- http://purl.org/ceu/simeon#Algorithm -->

    <owl:Class rdf:about="http://purl.org/ceu/simeon#Algorithm">
        <rdfs:label xml:lang="en">Algorithm</rdfs:label>
        <rdfs:label xml:lang="es">Algoritmo</rdfs:label>
        <rdfs:comment xml:lang="en">An algorithm is a procedure for doing some calculations.</rdfs:comment>
        <rdfs:seeAlso xml:lang="en">The software ontology: http://theswo.sourceforge.net/</rdfs:seeAlso>
        <rdfs:seeAlso xml:lang="es">La ontología del software: http://theswo.sourceforge.net/</rdfs:seeAlso>
        <rdfs:comment xml:lang="es">Un algoritmo es un procedimiento para realizar unos cálculos.</rdfs:comment>
    </owl:Class>
    


    <!-- http://purl.org/ceu/simeon#ComparisonMeasure -->

    <owl:Class rdf:about="http://purl.org/ceu/simeon#ComparisonMeasure">
        <rdfs:label xml:lang="en">Comparison measure</rdfs:label>
        <rdfs:label xml:lang="es">Medida de comparación</rdfs:label>
        <rdfs:subClassOf>
            <owl:Restriction>
                <owl:onProperty rdf:resource="http://purl.org/ceu/simeon#hasValue"/>
                <owl:someValuesFrom>
                    <rdfs:Datatype>
                        <owl:onDatatype rdf:resource="&xsd;decimal"/>
                        <owl:withRestrictions rdf:parseType="Collection">
                            <rdf:Description>
                                <xsd:minInclusive rdf:datatype="&xsd;decimal">0</xsd:minInclusive>
                            </rdf:Description>
                        </owl:withRestrictions>
                    </rdfs:Datatype>
                </owl:someValuesFrom>
            </owl:Restriction>
        </rdfs:subClassOf>
        <rdfs:comment xml:lang="en">A comparison measure is a value that espresses the similarity or dissimilarity degree between two objects or data (literals).</rdfs:comment>
        <rdfs:comment xml:lang="es">Una medida de comparación es un valor que expresa el grado de similitud o disimilitud entre dos objetos o datos (literales).</rdfs:comment>
        <owl:disjointUnionOf rdf:parseType="Collection">
            <rdf:Description rdf:about="http://purl.org/ceu/simeon#DataComparisonMeasure"/>
            <rdf:Description rdf:about="http://purl.org/ceu/simeon#ObjectComparisonMeasure"/>
        </owl:disjointUnionOf>
    </owl:Class>
    


    <!-- http://purl.org/ceu/simeon#ComparisonMethod -->

    <owl:Class rdf:about="http://purl.org/ceu/simeon#ComparisonMethod">
        <rdfs:label xml:lang="en">Comparison method</rdfs:label>
        <rdfs:label xml:lang="es">Método de comparación</rdfs:label>
        <rdfs:comment xml:lang="en">A comparison method is a procedure to compare a source object or literal data with a target one that returns a real number, known as comparison measure, that expresses the similarity or dissimilarity degree of the source object or literal data with the target one.</rdfs:comment>
        <rdfs:comment xml:lang="es">Un método de comparación es un procedimiento para comparar un objeto o dato literal origen con otro destino que devuelve un número real, conocido como medida de comparación, que expresa el grado de similitud o disimilitud del objeto o dato origen con el destino.</rdfs:comment>
        <owl:disjointUnionOf rdf:parseType="Collection">
            <rdf:Description rdf:about="http://purl.org/ceu/simeon#DataComparisonMethod"/>
            <rdf:Description rdf:about="http://purl.org/ceu/simeon#ObjectComparisonMethod"/>
        </owl:disjointUnionOf>
    </owl:Class>
    


    <!-- http://purl.org/ceu/simeon#DataComparisonMeasure -->

    <owl:Class rdf:about="http://purl.org/ceu/simeon#DataComparisonMeasure">
        <rdfs:label xml:lang="en">Data comparison measure</rdfs:label>
        <rdfs:label xml:lang="es">Medida de comparación de datos</rdfs:label>
        <rdfs:subClassOf rdf:resource="http://purl.org/ceu/simeon#ComparisonMeasure"/>
        <rdfs:subClassOf>
            <owl:Restriction>
                <owl:onProperty rdf:resource="http://purl.org/ceu/simeon#hasSourceData"/>
                <owl:someValuesFrom rdf:resource="&rdfs;Literal"/>
            </owl:Restriction>
        </rdfs:subClassOf>
        <rdfs:subClassOf>
            <owl:Restriction>
                <owl:onProperty rdf:resource="http://purl.org/ceu/simeon#hasTargetData"/>
                <owl:someValuesFrom rdf:resource="&rdfs;Literal"/>
            </owl:Restriction>
        </rdfs:subClassOf>
        <rdfs:subClassOf>
            <owl:Restriction>
                <owl:onProperty rdf:resource="http://purl.org/ceu/simeon#usesComparisonMethod"/>
                <owl:someValuesFrom rdf:resource="http://purl.org/ceu/simeon#DataComparisonMethod"/>
            </owl:Restriction>
        </rdfs:subClassOf>
        <owl:disjointWith rdf:resource="http://purl.org/ceu/simeon#ObjectComparisonMeasure"/>
        <rdfs:comment xml:lang="en">A comparison measure is a value that espresses the similarity or dissimilarity degree between two simple data (literals): booleans, numbers, dates, strings, etc.</rdfs:comment>
        <rdfs:comment xml:lang="es">Una medida de comparación es un valor que expresa el grado de similitud o disimilitud entre dos datos simples (literales): booleanos, números, fechas, cadenas, etc.</rdfs:comment>
    </owl:Class>
    


    <!-- http://purl.org/ceu/simeon#DataComparisonMethod -->

    <owl:Class rdf:about="http://purl.org/ceu/simeon#DataComparisonMethod">
        <rdfs:label xml:lang="en">Data comparison method</rdfs:label>
        <rdfs:label xml:lang="es">Método de comparación de datos</rdfs:label>
        <rdfs:subClassOf rdf:resource="http://purl.org/ceu/simeon#ComparisonMethod"/>
        <owl:disjointWith rdf:resource="http://purl.org/ceu/simeon#ObjectComparisonMethod"/>
        <rdfs:comment xml:lang="en">A comparison method is a procedure to compare a source literal data with a target literal data that returns a real number, known as comparison measure, that expresses the similarity or dissimilarity degree of the source literal data with the target one.</rdfs:comment>
        <rdfs:comment xml:lang="es">Un método de comparación es un procedimiento para comparar un dato literal origen con otro destino que devuelve un número real, conocido como medida de comparación, que expresa el grado de similitud o disimilitud del dato literal origen con el destino.</rdfs:comment>
    </owl:Class>
    


    <!-- http://purl.org/ceu/simeon#DissimilarityFunction -->

    <owl:Class rdf:about="http://purl.org/ceu/simeon#DissimilarityFunction">
        <rdfs:label xml:lang="en">Dissimilarity function</rdfs:label>
        <rdfs:label xml:lang="es">Función de disimilitud</rdfs:label>
        <rdfs:subClassOf rdf:resource="http://purl.org/ceu/simeon#ComparisonMethod"/>
        <rdfs:comment xml:lang="en">A dissimilarity function is a real function that associates to every pair of objects in a domain, a real number that expresses the unlikeness, dissimilarity or distance between the two objects according to some of their features, and satisfies the following axioms:
1- Non-negativity: d(x,y) ≥ 0 for all x, y. 
2- Minimality: d(x,x) = 0 for all x.</rdfs:comment>
        <rdfs:comment xml:lang="es">Una función de disimilitud es una función real que asocia a cada par de elementos de un mismo dominio, un número real que expresa el grado de desemejanza, disimilitud o distancia entre los dos objetos de acuerdo a alguna de sus características, y satisface los siguientes axiomas:
1- No negatividad: d(x, y) ≥ 0 para todo x, y. 
2- Minimalidad: d(x, x) = 0  para todo x.</rdfs:comment>
    </owl:Class>
    


    <!-- http://purl.org/ceu/simeon#DissimilarityMeasure -->

    <owl:Class rdf:about="http://purl.org/ceu/simeon#DissimilarityMeasure">
        <rdfs:label xml:lang="en">Dissimilarity measure</rdfs:label>
        <rdfs:label xml:lang="es">Medida de disimilitud</rdfs:label>
        <rdfs:subClassOf rdf:resource="http://purl.org/ceu/simeon#ObjectiveComparisonMeasure"/>
        <rdfs:subClassOf>
            <owl:Restriction>
                <owl:onProperty rdf:resource="http://purl.org/ceu/simeon#usesComparisonMethod"/>
                <owl:someValuesFrom rdf:resource="http://purl.org/ceu/simeon#DissimilarityFunction"/>
            </owl:Restriction>
        </rdfs:subClassOf>
        <owl:disjointWith rdf:resource="http://purl.org/ceu/simeon#SimilarityMeasure"/>
        <rdfs:comment xml:lang="en">A dissimilarity measure is a number that expresses the dissimilarity or discrepance degree between two objects, calculated with a dissimilarity function, that is, a real function d that satisfies the following axioms:
1- Non-negativity: d(x,y) ≥ 0 for all x, y. 
2- Minimality: d(x,x) = 0 for all x.</rdfs:comment>
        <rdfs:comment xml:lang="es">Una medida de disimilitud es un número que establece el grado de disimilitud o discrepancia entre dos objetos, calculado con una función de disimilitud, es decir, una función real d que satisface los siguientes axiomas:
1- No negatividad: d(x, y) ≥ 0 para todo x, y. 
2- Minimalidad: d(x, x) = 0  para todo x.</rdfs:comment>
    </owl:Class>
    


    <!-- http://purl.org/ceu/simeon#DistanceFunction -->

    <owl:Class rdf:about="http://purl.org/ceu/simeon#DistanceFunction">
        <rdfs:label xml:lang="en">Distance function</rdfs:label>
        <rdfs:label xml:lang="es">Función de distancia</rdfs:label>
        <rdfs:subClassOf rdf:resource="http://purl.org/ceu/simeon#SymmetricDissimilarityFunction"/>
        <rdfs:comment xml:lang="en">A distance function is a dissimilarity function d that satisfies the following axioms:
1- Non negativity: d(x,y) ≥ 0 for all x,y.
2- Coincidence: d(x,y) = 0 if and only if x=y. 
3- Symmetry: d(x,y) = d(y,x) for all x,y.
4- Triangle inequality: d(x,z) ≤ d(x,y) + d(y,z) for all x,y,z.</rdfs:comment>
        <rdfs:comment xml:lang="es">Una función de distancia es una función de disimilitud d que satisface los siguientes axiomas:
1- No negatividad: d(x,y) ≥ 0 para todo x,y.
2- Coincidencia: d(x,y) = 0 si y sólo si x=y.
3- Simetría: d(x,y) = d(y,x) para todo x,y.
4- Desigualdad triangular: d(x,z) ≤ d(x,y) + d(y,z) para todo x,y,z.</rdfs:comment>
    </owl:Class>
    


    <!-- http://purl.org/ceu/simeon#DistanceMeasure -->

    <owl:Class rdf:about="http://purl.org/ceu/simeon#DistanceMeasure">
        <rdfs:label xml:lang="en">Distance measure</rdfs:label>
        <rdfs:label xml:lang="es">Medida de distancia</rdfs:label>
        <rdfs:subClassOf rdf:resource="http://purl.org/ceu/simeon#SymmetricDissimilarityMeasure"/>
        <rdfs:subClassOf>
            <owl:Restriction>
                <owl:onProperty rdf:resource="http://purl.org/ceu/simeon#usesComparisonMethod"/>
                <owl:someValuesFrom rdf:resource="http://purl.org/ceu/simeon#DistanceFunction"/>
            </owl:Restriction>
        </rdfs:subClassOf>
        <rdfs:comment xml:lang="en">A distance measure is a value that expresses the degree of dissimilarity between two objects calculated with a distance funcion, that is, a real function d that satisfies the following axioms:
1- Non negativity: d(x,y) ≥ 0 for all x,y.
2- Coincidence: d(x,y) = 0 if and only if x=y. 
3- Symmetry: d(x,y) = d(y,x) for all x,y.
4- Triangle inequality: d(x,z) ≤ d(x,y) + d(y,z) for all x,y,z.</rdfs:comment>
        <rdfs:comment xml:lang="es">Una medida de distancia es un número que expresa el grado de disimilitud entre dos objetos calculado con una función de distancia d, es decir, una función real d que satisface los siguientes axiomas:
1- No negatividad: d(x,y) ≥ 0 para todo x,y.
2- Coincidencia: d(x,y) = 0 si y sólo si x=y.
3- Simetría: d(x,y) = d(y,x) para todo x,y.
4- Desigualdad triangular: d(x,z) ≤ d(x,y) + d(y,z) para todo x,y,z.</rdfs:comment>
    </owl:Class>
    


    <!-- http://purl.org/ceu/simeon#NormalizedComparisonMeasure -->

    <owl:Class rdf:about="http://purl.org/ceu/simeon#NormalizedComparisonMeasure">
        <rdfs:label xml:lang="en">Normalized similarity measure</rdfs:label>
        <rdfs:label xml:lang="es">Medida de comparación normalizada</rdfs:label>
        <owl:equivalentClass>
            <owl:Class>
                <owl:intersectionOf rdf:parseType="Collection">
                    <rdf:Description rdf:about="http://purl.org/ceu/simeon#ComparisonMeasure"/>
                    <owl:Restriction>
                        <owl:onProperty rdf:resource="http://purl.org/ceu/simeon#hasValue"/>
                        <owl:allValuesFrom>
                            <rdfs:Datatype>
                                <owl:onDatatype rdf:resource="&xsd;decimal"/>
                                <owl:withRestrictions rdf:parseType="Collection">
                                    <rdf:Description>
                                        <xsd:maxInclusive rdf:datatype="&xsd;integer">1</xsd:maxInclusive>
                                    </rdf:Description>
                                    <rdf:Description>
                                        <xsd:minInclusive rdf:datatype="&xsd;integer">0</xsd:minInclusive>
                                    </rdf:Description>
                                </owl:withRestrictions>
                            </rdfs:Datatype>
                        </owl:allValuesFrom>
                    </owl:Restriction>
                </owl:intersectionOf>
            </owl:Class>
        </owl:equivalentClass>
        <rdfs:subClassOf>
            <owl:Restriction>
                <owl:onProperty rdf:resource="http://purl.org/ceu/simeon#usesComparisonMethod"/>
                <owl:someValuesFrom rdf:resource="http://purl.org/ceu/simeon#NormalizedComparisonMethod"/>
            </owl:Restriction>
        </rdfs:subClassOf>
        <rdfs:comment xml:lang="en">A normalized comparison measure is a comparison measure in te real interval [0,1].</rdfs:comment>
        <rdfs:comment xml:lang="es">Una medida de comparación normalizada es una medida en el intervalo real [0,1].</rdfs:comment>
    </owl:Class>
    


    <!-- http://purl.org/ceu/simeon#NormalizedComparisonMethod -->

    <owl:Class rdf:about="http://purl.org/ceu/simeon#NormalizedComparisonMethod">
        <rdfs:label xml:lang="en">Normalized comparison method</rdfs:label>
        <rdfs:label xml:lang="es">Método de comparación normalizado</rdfs:label>
        <rdfs:subClassOf rdf:resource="http://purl.org/ceu/simeon#ComparisonMethod"/>
        <rdfs:comment xml:lang="en">A normalized comparison method is a comparison method that returns a number in the real interval [0,1].</rdfs:comment>
        <rdfs:comment xml:lang="es">Un método de comparación normalizado es un método de comparación que devuelve un número real en el intervalo [0,1].</rdfs:comment>
    </owl:Class>
    


    <!-- http://purl.org/ceu/simeon#NormalizedDissimilarityFunction -->

    <owl:Class rdf:about="http://purl.org/ceu/simeon#NormalizedDissimilarityFunction">
        <rdfs:label xml:lang="en">Normalized dissimilarity function</rdfs:label>
        <rdfs:label xml:lang="es">Función de disimilitud normalizada</rdfs:label>
        <owl:equivalentClass>
            <owl:Class>
                <owl:intersectionOf rdf:parseType="Collection">
                    <rdf:Description rdf:about="http://purl.org/ceu/simeon#DissimilarityFunction"/>
                    <rdf:Description rdf:about="http://purl.org/ceu/simeon#NormalizedComparisonMethod"/>
                </owl:intersectionOf>
            </owl:Class>
        </owl:equivalentClass>
        <rdfs:comment xml:lang="en">A normalized dissimilarity function is a dissimilarity function with range the real inteval [0,1], that is, that returns values between 0 and 1.</rdfs:comment>
        <rdfs:comment xml:lang="es">Una función de disimilitud normalizada es una función de disimilitud con rango el intervalo real [0,1], es decir, que devuelve valores entre 0 y 1.</rdfs:comment>
    </owl:Class>
    


    <!-- http://purl.org/ceu/simeon#NormalizedDissimilarityMeasure -->

    <owl:Class rdf:about="http://purl.org/ceu/simeon#NormalizedDissimilarityMeasure">
        <rdfs:label xml:lang="en">Normalized dissimilarity measure</rdfs:label>
        <rdfs:label xml:lang="es">Medida de disimilitud normalizada</rdfs:label>
        <owl:equivalentClass>
            <owl:Class>
                <owl:intersectionOf rdf:parseType="Collection">
                    <rdf:Description rdf:about="http://purl.org/ceu/simeon#DissimilarityMeasure"/>
                    <rdf:Description rdf:about="http://purl.org/ceu/simeon#NormalizedComparisonMeasure"/>
                </owl:intersectionOf>
            </owl:Class>
        </owl:equivalentClass>
        <rdfs:comment xml:lang="en">A normalized dissimilarity measure is a dissimilarity measure in the real interval [0,1].</rdfs:comment>
        <rdfs:comment xml:lang="es">Una medida de disimilitud normalizada es una medida de disimilitud en el intervalo real [0,1].</rdfs:comment>
    </owl:Class>
    


    <!-- http://purl.org/ceu/simeon#NormalizedDistanceFunction -->

    <owl:Class rdf:about="http://purl.org/ceu/simeon#NormalizedDistanceFunction">
        <rdfs:label xml:lang="en">Normalized distance function</rdfs:label>
        <rdfs:label xml:lang="es">Función de distancia normalizada</rdfs:label>
        <owl:equivalentClass>
            <owl:Class>
                <owl:intersectionOf rdf:parseType="Collection">
                    <rdf:Description rdf:about="http://purl.org/ceu/simeon#DistanceFunction"/>
                    <rdf:Description rdf:about="http://purl.org/ceu/simeon#NormalizedComparisonMethod"/>
                </owl:intersectionOf>
            </owl:Class>
        </owl:equivalentClass>
        <rdfs:comment xml:lang="en">A normalized distance function is a distance function with range the real inteval [0,1], that is, that returns values between 0 and 1</rdfs:comment>
        <rdfs:comment xml:lang="es">Una función de distancia normalizada es una función de distancia con rango el intervalo real [0,1], es decir, que devuelve valores entre 0 y 1</rdfs:comment>
    </owl:Class>
    


    <!-- http://purl.org/ceu/simeon#NormalizedDistanceMeasure -->

    <owl:Class rdf:about="http://purl.org/ceu/simeon#NormalizedDistanceMeasure">
        <rdfs:label xml:lang="en">Normalized distance measure</rdfs:label>
        <rdfs:label xml:lang="es">Medida de distancia normalizada</rdfs:label>
        <owl:equivalentClass>
            <owl:Class>
                <owl:intersectionOf rdf:parseType="Collection">
                    <rdf:Description rdf:about="http://purl.org/ceu/simeon#DistanceMeasure"/>
                    <rdf:Description rdf:about="http://purl.org/ceu/simeon#NormalizedComparisonMeasure"/>
                </owl:intersectionOf>
            </owl:Class>
        </owl:equivalentClass>
        <rdfs:comment xml:lang="en">A normalized distance measure is a distance measure in the real interval [0,1].</rdfs:comment>
        <rdfs:comment xml:lang="es">Una medida de distancia normalizada es una medida de distancia en el intervalo real [0,1].</rdfs:comment>
    </owl:Class>
    


    <!-- http://purl.org/ceu/simeon#NormalizedSimilarityFunction -->

    <owl:Class rdf:about="http://purl.org/ceu/simeon#NormalizedSimilarityFunction">
        <rdfs:label xml:lang="en">Normalized similarity function</rdfs:label>
        <rdfs:label xml:lang="es">Función de similitud normalizada</rdfs:label>
        <owl:equivalentClass>
            <owl:Class>
                <owl:intersectionOf rdf:parseType="Collection">
                    <rdf:Description rdf:about="http://purl.org/ceu/simeon#NormalizedComparisonMethod"/>
                    <rdf:Description rdf:about="http://purl.org/ceu/simeon#SimilarityFunction"/>
                </owl:intersectionOf>
            </owl:Class>
        </owl:equivalentClass>
        <rdfs:comment xml:lang="en">A normalized similarity function is a similarity function with range the real interval [0,1], that is, that returns values between 0 and 1.</rdfs:comment>
        <rdfs:comment xml:lang="es">Una función de similitud normalizada es una función de similitud cuyo rango es el intervalo real [0,1], es decir que devuelve valores entre 0 y 1.</rdfs:comment>
    </owl:Class>
    


    <!-- http://purl.org/ceu/simeon#NormalizedSimilarityMeasure -->

    <owl:Class rdf:about="http://purl.org/ceu/simeon#NormalizedSimilarityMeasure">
        <rdfs:label xml:lang="en">Normalized similarity measure</rdfs:label>
        <rdfs:label xml:lang="es">Medida de similitud normalizada</rdfs:label>
        <owl:equivalentClass>
            <owl:Class>
                <owl:intersectionOf rdf:parseType="Collection">
                    <rdf:Description rdf:about="http://purl.org/ceu/simeon#NormalizedComparisonMeasure"/>
                    <rdf:Description rdf:about="http://purl.org/ceu/simeon#SimilarityMeasure"/>
                </owl:intersectionOf>
            </owl:Class>
        </owl:equivalentClass>
        <rdfs:comment xml:lang="en">A normalized similarity measure is a similiarity measure in the real interval [0,1].</rdfs:comment>
        <rdfs:comment xml:lang="es">Una medida de similitud normalizada es una medida de similitud en el intervalo real [0,1].</rdfs:comment>
    </owl:Class>
    


    <!-- http://purl.org/ceu/simeon#ObjectComparisonMeasure -->

    <owl:Class rdf:about="http://purl.org/ceu/simeon#ObjectComparisonMeasure">
        <rdfs:label xml:lang="en">Object comparison measure</rdfs:label>
        <rdfs:label xml:lang="es">Medida de comparación de objetos</rdfs:label>
        <rdfs:subClassOf rdf:resource="http://purl.org/ceu/simeon#ComparisonMeasure"/>
        <rdfs:subClassOf>
            <owl:Restriction>
                <owl:onProperty rdf:resource="http://purl.org/ceu/simeon#hasTargetObject"/>
                <owl:someValuesFrom rdf:resource="&owl;Thing"/>
            </owl:Restriction>
        </rdfs:subClassOf>
        <rdfs:subClassOf>
            <owl:Restriction>
                <owl:onProperty rdf:resource="http://purl.org/ceu/simeon#hasSourceObject"/>
                <owl:someValuesFrom rdf:resource="&owl;Thing"/>
            </owl:Restriction>
        </rdfs:subClassOf>
        <rdfs:comment xml:lang="en">A comparison measure is a value that espresses the similarity or dissimilarity degree between two objects that are not literals.</rdfs:comment>
        <rdfs:comment xml:lang="es">Una medida de comparación es un valor que expresa el grado de similitud o disimilitud entre dos objetos que no son literales.</rdfs:comment>
    </owl:Class>
    


    <!-- http://purl.org/ceu/simeon#ObjectComparisonMethod -->

    <owl:Class rdf:about="http://purl.org/ceu/simeon#ObjectComparisonMethod">
        <rdfs:label xml:lang="en">Object comparison method</rdfs:label>
        <rdfs:label xml:lang="es">Método de comparación de objetos</rdfs:label>
        <rdfs:subClassOf rdf:resource="http://purl.org/ceu/simeon#ComparisonMethod"/>
        <rdfs:comment xml:lang="en">A comparison method is a procedure to compare a source object (non literal) with a target one, that returns a real number, known as comparison measure, that expresses the similarity or dissimilarity degree of the source object with the target one.</rdfs:comment>
        <rdfs:comment xml:lang="es">Un método de comparación es un procedimiento para comparar un objeto origen con otro destino, que devuelve un número real, conocido como medida de comparación, que expresa el grado de similitud o disimilitud del objeto origen con el destino.</rdfs:comment>
    </owl:Class>
    


    <!-- http://purl.org/ceu/simeon#ObjectiveComparisonMeasure -->

    <owl:Class rdf:about="http://purl.org/ceu/simeon#ObjectiveComparisonMeasure">
        <rdfs:label xml:lang="en">Objective comparison measure</rdfs:label>
        <rdfs:label xml:lang="es">Medida de comparación objetiva</rdfs:label>
        <rdfs:subClassOf rdf:resource="http://purl.org/ceu/simeon#ComparisonMeasure"/>
        <owl:disjointWith rdf:resource="http://purl.org/ceu/simeon#SubjectiveComparisonMeasure"/>
        <rdfs:comment xml:lang="en">An objective comparison measure is a comparison measure calculated with an objective comparison method, that is, a method that always returns the same value when applied to the same objects.</rdfs:comment>
        <rdfs:comment xml:lang="es">Una medida de comparación objetiva es una medida de comparación realizada con un método de comparación objetivo, es decir, un método que siempre da el mismo resultado cuando se aplica a los mismos objetos.</rdfs:comment>
    </owl:Class>
    


    <!-- http://purl.org/ceu/simeon#SimilarityFunction -->

    <owl:Class rdf:about="http://purl.org/ceu/simeon#SimilarityFunction">
        <rdfs:label xml:lang="en">Similarity function</rdfs:label>
        <rdfs:label xml:lang="es">Función de similitud</rdfs:label>
        <rdfs:subClassOf rdf:resource="http://purl.org/ceu/simeon#ComparisonMethod"/>
        <rdfs:comment xml:lang="en">A similarity function is a real function that associates to every pair of objects in a domain, a real number that expresses the likeness, similarity or proximity degree between the two objects according to some of their features, and satisfies the following axioms:
1- Non-negativity: s(x, y) ≥ 0 for all x, y. 
2- Maximality: s(x, x) ≥ s(x,y) for all x, y.</rdfs:comment>
        <rdfs:comment xml:lang="es">Una función de similitud es una función real s que asocia a cada par de objetos de un mismo dominio, un número real que expresa el grado de parecido,  semejanza o proximidad entre los dos objetos de acuerdo a alguna de sus características, y satisface los siguientes axiomas:
1- No negatividad: s(x, y) ≥ 0 para todo x, y. 
2- Maximalidad: s(x, x) ≥ s(x,y) para todo x, y.</rdfs:comment>
    </owl:Class>
    


    <!-- http://purl.org/ceu/simeon#SimilarityMeasure -->

    <owl:Class rdf:about="http://purl.org/ceu/simeon#SimilarityMeasure">
        <rdfs:label xml:lang="en">Similarity measure</rdfs:label>
        <rdfs:label xml:lang="es">Medida de similitud</rdfs:label>
        <rdfs:subClassOf rdf:resource="http://purl.org/ceu/simeon#ObjectiveComparisonMeasure"/>
        <rdfs:subClassOf>
            <owl:Restriction>
                <owl:onProperty rdf:resource="http://purl.org/ceu/simeon#usesComparisonMethod"/>
                <owl:someValuesFrom rdf:resource="http://purl.org/ceu/simeon#SimilarityFunction"/>
            </owl:Restriction>
        </rdfs:subClassOf>
        <rdfs:comment xml:lang="en">A similarity measure is a number that expresses the similarity degree between two objects, calculated with a similarity function, that is, a real function s that satisfies the following axioms:
1- Non-negativity: s(x, y) ≥ 0 for all x, y. 
2- Maximality: s(x, x) ≥ s(x,y) for all x, y.</rdfs:comment>
        <rdfs:comment xml:lang="es">Una medida de similitud es un número que establece el grado de semejanza o similitud entre dos objetos, calculado con una función de similitud, es decir, una función real s que satisface los siguientes axiomas:
1- No negatividad: s(x, y) ≥ 0 para todo x, y. 
2- Maximalidad: s(x, x) ≥ s(x,y) para todo x, y.</rdfs:comment>
    </owl:Class>
    


    <!-- http://purl.org/ceu/simeon#SubjectiveComparisonMeasure -->

    <owl:Class rdf:about="http://purl.org/ceu/simeon#SubjectiveComparisonMeasure">
        <rdfs:label xml:lang="en">Subjective comparison measure</rdfs:label>
        <rdfs:label xml:lang="es">Medida de comparación subjetiva</rdfs:label>
        <rdfs:subClassOf rdf:resource="http://purl.org/ceu/simeon#ComparisonMeasure"/>
        <rdfs:comment xml:lang="en">A subjective comparison measure is a measure obtained with a subjective comparison method, that is, based on the perception, feelings or opinion of a person.</rdfs:comment>
        <rdfs:comment xml:lang="es">Una medida de comparación subjetiva es una medida realizada con un método de comparación subjetivo, es decir, basado en la percepción, sentimientos u opinión de una persona.</rdfs:comment>
    </owl:Class>
    


    <!-- http://purl.org/ceu/simeon#SymmetricComparisonMeasure -->

    <owl:Class rdf:about="http://purl.org/ceu/simeon#SymmetricComparisonMeasure">
        <rdfs:label xml:lang="en">Symmetric comparison measure</rdfs:label>
        <rdfs:label xml:lang="es">Medida de comaración simétrica</rdfs:label>
        <rdfs:subClassOf rdf:resource="http://purl.org/ceu/simeon#ComparisonMeasure"/>
        <rdfs:subClassOf>
            <owl:Restriction>
                <owl:onProperty rdf:resource="http://purl.org/ceu/simeon#usesComparisonMethod"/>
                <owl:someValuesFrom rdf:resource="http://purl.org/ceu/simeon#SymmetricComparisonMethod"/>
            </owl:Restriction>
        </rdfs:subClassOf>
        <rdfs:comment xml:lang="en">A symmetric comparison measure is a comparison measure calculated with a symmetric comparison function, that is, a real function c that satisfies the symmetry axiom:
c(x,y) = c(y,x) for all x,y.</rdfs:comment>
        <rdfs:comment xml:lang="es">Una medida de comparación simétrica es una medida de comparación calculada con una función de comparación simétrica, es decir, una función real c que satisface el axioma de simetría:
c(x,y) = c(y,x) para todo x,y.</rdfs:comment>
    </owl:Class>
    


    <!-- http://purl.org/ceu/simeon#SymmetricComparisonMethod -->

    <owl:Class rdf:about="http://purl.org/ceu/simeon#SymmetricComparisonMethod">
        <rdfs:label xml:lang="en">Symmetric comparison method</rdfs:label>
        <rdfs:label xml:lang="es">Método de comparación simétrico</rdfs:label>
        <rdfs:subClassOf rdf:resource="http://purl.org/ceu/simeon#ComparisonMethod"/>
        <rdfs:comment xml:lang="en">A symmetric comparison method is a comparison method or function c that satisfies the symmetry axiom:
c(x,y) = c(y,x) for all x,y.</rdfs:comment>
        <rdfs:comment xml:lang="es">Un método de comparación simétrico es un método de comparación o función c que satisface el axioma de simetría:
c(x,y) = c(y,x) para todo x,y.</rdfs:comment>
    </owl:Class>
    


    <!-- http://purl.org/ceu/simeon#SymmetricDissimilarityFunction -->

    <owl:Class rdf:about="http://purl.org/ceu/simeon#SymmetricDissimilarityFunction">
        <rdfs:label xml:lang="en">Symmetric dissimilarity function</rdfs:label>
        <rdfs:label xml:lang="es">Función de disimilitud simétrica</rdfs:label>
        <owl:equivalentClass>
            <owl:Class>
                <owl:intersectionOf rdf:parseType="Collection">
                    <rdf:Description rdf:about="http://purl.org/ceu/simeon#DissimilarityFunction"/>
                    <rdf:Description rdf:about="http://purl.org/ceu/simeon#SymmetricComparisonMethod"/>
                </owl:intersectionOf>
            </owl:Class>
        </owl:equivalentClass>
        <rdfs:comment xml:lang="en">A symmetric dissimilarity function is a dissimilarity function d that satisfies the symmetry axiom
d(x,y) = d(y,x) for all x,y.</rdfs:comment>
        <rdfs:comment xml:lang="es">Una función de disimilitud simétrica es una función de disimilitud d que satisface el axioma de simetría
d(x,y) = d(y,x) para todo x,y.</rdfs:comment>
    </owl:Class>
    


    <!-- http://purl.org/ceu/simeon#SymmetricDissimilarityMeasure -->

    <owl:Class rdf:about="http://purl.org/ceu/simeon#SymmetricDissimilarityMeasure">
        <rdfs:label xml:lang="en">Symmetric dissimilarity measure</rdfs:label>
        <rdfs:label xml:lang="es">Medida de disimilitud simétrica</rdfs:label>
        <rdfs:subClassOf rdf:resource="http://purl.org/ceu/simeon#DissimilarityMeasure"/>
        <rdfs:subClassOf rdf:resource="http://purl.org/ceu/simeon#SymmetricComparisonMeasure"/>
        <rdfs:comment xml:lang="en">A symmetric dissimilarity measure is a dissimilarity measure calculated with a symmetric dissimilarity function, that is, a real function d that satisfies the symmetry axiom:
d(x,y) = d(y,x) for all x,y.</rdfs:comment>
        <rdfs:comment xml:lang="es">Una medida de disimilitud simétrica es una medida de disimilitud calculada con una función de disimilitud simétrica, es decir, una función real d que satisface el axioma de simetría:
d(x,y) = d(y,x) para todo x,y.</rdfs:comment>
    </owl:Class>
    


    <!-- http://purl.org/ceu/simeon#SymmetricSimilarityFunction -->

    <owl:Class rdf:about="http://purl.org/ceu/simeon#SymmetricSimilarityFunction">
        <rdfs:label xml:lang="en">Symmetric similarity function</rdfs:label>
        <rdfs:label xml:lang="es">Función de similitud simétrica</rdfs:label>
        <owl:equivalentClass>
            <owl:Class>
                <owl:intersectionOf rdf:parseType="Collection">
                    <rdf:Description rdf:about="http://purl.org/ceu/simeon#SimilarityFunction"/>
                    <rdf:Description rdf:about="http://purl.org/ceu/simeon#SymmetricComparisonMethod"/>
                </owl:intersectionOf>
            </owl:Class>
        </owl:equivalentClass>
        <rdfs:comment xml:lang="en">A symmetric similarity function is a similarity function that satisfies the symmetry axiom
s(x,y) = s(y,x) for all x,y.</rdfs:comment>
        <rdfs:comment xml:lang="es">Una función de similitud simétrica es una función de similitud s que satisface el axioma de simetría
s(x,y) = s(y,x) para todo x,y.</rdfs:comment>
    </owl:Class>
    


    <!-- http://purl.org/ceu/simeon#SymmetricSimilarityMeasure -->

    <owl:Class rdf:about="http://purl.org/ceu/simeon#SymmetricSimilarityMeasure">
        <rdfs:label xml:lang="en">Symmetric similarity measure</rdfs:label>
        <rdfs:label xml:lang="es">Medida de similitud simétrica</rdfs:label>
        <rdfs:subClassOf rdf:resource="http://purl.org/ceu/simeon#SimilarityMeasure"/>
        <rdfs:subClassOf rdf:resource="http://purl.org/ceu/simeon#SymmetricComparisonMeasure"/>
        <rdfs:comment xml:lang="en">A symmetric similarity measure is a similarity measure calculated with a symmetric similarity function, that is, a real function s that satisfies the symmetry axiom:
s(x,y) = s(y,x) for all x,y.</rdfs:comment>
        <rdfs:comment xml:lang="es">Una medida de similitud simétrica es una medida de similitud calculada con una función de similitud simétrica, es decir, una función real s que satisface el axioma de simetría:
s(x,y) = s(y,x) para todo x,y.</rdfs:comment>
    </owl:Class>
    


    <!-- http://purl.org/dc/terms/Agent -->

    <owl:Class rdf:about="http://purl.org/dc/terms/Agent">
        <rdfs:label xml:lang="en">Agent</rdfs:label>
        <rdfs:label xml:lang="es">Agente</rdfs:label>
        <rdfs:comment xml:lang="en">An agent is an entity (person or artefact) capable of acting and doing things.</rdfs:comment>
        <rdfs:seeAlso xml:lang="en">The Dublin Core Ontology: http://dublincore.org/documents/dcmi-terms/</rdfs:seeAlso>
        <rdfs:seeAlso xml:lang="es">La ontología Dublin Core: http://dublincore.org/documents/dcmi-terms/</rdfs:seeAlso>
        <rdfs:comment xml:lang="es">Un agente es una entidad (persona o artefacto) capaz de actuar y hacer cosas.</rdfs:comment>
    </owl:Class>
    


    <!-- http://purl.org/dc/terms/BibliographicResource -->

    <owl:Class rdf:about="http://purl.org/dc/terms/BibliographicResource">
        <rdfs:label xml:lang="en">Bibliographic resource</rdfs:label>
        <rdfs:label xml:lang="es">Recurso bibliográfico</rdfs:label>
        <rdfs:comment xml:lang="en">A bibliographic resource is a publication (article, book, web page, etc.)</rdfs:comment>
        <rdfs:seeAlso xml:lang="en">The Dublin Core Ontology: http://dublincore.org/documents/dcmi-terms/</rdfs:seeAlso>
        <rdfs:seeAlso xml:lang="es">La ontología Dublin Core: http://dublincore.org/documents/dcmi-terms/</rdfs:seeAlso>
        <rdfs:comment xml:lang="es">Un recurso bibliográfico es una publicación (artículo, libro, página web, etc).</rdfs:comment>
    </owl:Class>
    


    <!-- 
    ///////////////////////////////////////////////////////////////////////////////////////
    //
    // Individuals
    //
    ///////////////////////////////////////////////////////////////////////////////////////
     -->

    


    <!-- http://purl.org/ceu/simeon#dataIdentitySimilarityFunction -->

    <owl:NamedIndividual rdf:about="http://purl.org/ceu/simeon#dataIdentitySimilarityFunction">
        <rdf:type rdf:resource="http://purl.org/ceu/simeon#NormalizedSimilarityFunction"/>
        <rdf:type rdf:resource="http://purl.org/ceu/simeon#SymmetricSimilarityFunction"/>
    </owl:NamedIndividual>
    


    <!-- http://purl.org/ceu/simeon#objectIdentitySimilarityFunction -->

    <owl:NamedIndividual rdf:about="http://purl.org/ceu/simeon#objectIdentitySimilarityFunction">
        <rdf:type rdf:resource="http://purl.org/ceu/simeon#NormalizedSimilarityFunction"/>
        <rdf:type rdf:resource="http://purl.org/ceu/simeon#SymmetricSimilarityFunction"/>
        <rdfs:label xml:lang="en">identity similarity function</rdfs:label>
        <rdfs:label xml:lang="es">función de similitud identidad</rdfs:label>
        <rdfs:comment xml:lang="en">The identity similarity function is a normalized similarity function s such that
s(x,y)=1 if x=y 
s(x,y)=0 if x≠y</rdfs:comment>
        <rdfs:comment xml:lang="es">Una función de similitud simétrica es una función de similitud s que satisface el axioma de simetría
s(x,y) = s(y,x) para todo x,y.</rdfs:comment>
    </owl:NamedIndividual>
    


    <!-- 
    ///////////////////////////////////////////////////////////////////////////////////////
    //
    // Annotations
    //
    ///////////////////////////////////////////////////////////////////////////////////////
     -->

    <rdf:Description rdf:about="&owl;topDataProperty">
        <rdfs:label xml:lang="en">compares entity</rdfs:label>
        <rdfs:label xml:lang="es">compara entidad</rdfs:label>
        <rdfs:comment xml:lang="en">Property that relates a comparison method with an entity that is compared with other using that method.</rdfs:comment>
        <rdfs:comment xml:lang="es">Propiedad que relaciona un método de comparación con una entidad que ha sido comparada con otra utilizando ese método.</rdfs:comment>
    </rdf:Description>
    


    <!-- 
    ///////////////////////////////////////////////////////////////////////////////////////
    //
    // Rules
    //
    ///////////////////////////////////////////////////////////////////////////////////////
     -->

    <rdf:Description rdf:about="urn:swrl#similarity">
        <rdf:type rdf:resource="&swrl;Variable"/>
    </rdf:Description>
    <rdf:Description rdf:about="urn:swrl#individual1">
        <rdf:type rdf:resource="&swrl;Variable"/>
    </rdf:Description>
    <rdf:Description rdf:about="urn:swrl#individual2">
        <rdf:type rdf:resource="&swrl;Variable"/>
    </rdf:Description>
    <rdf:Description rdf:about="urn:swrl#literal2">
        <rdf:type rdf:resource="&swrl;Variable"/>
    </rdf:Description>
    <rdf:Description rdf:about="urn:swrl#literal1">
        <rdf:type rdf:resource="&swrl;Variable"/>
    </rdf:Description>
    <rdf:Description rdf:about="urn:swrl#measure1">
        <rdf:type rdf:resource="&swrl;Variable"/>
    </rdf:Description>
    <rdf:Description rdf:about="urn:swrl#method">
        <rdf:type rdf:resource="&swrl;Variable"/>
    </rdf:Description>
    <rdf:Description rdf:about="urn:swrl#value">
        <rdf:type rdf:resource="&swrl;Variable"/>
    </rdf:Description>
    <rdf:Description rdf:about="urn:swrl#measure2">
        <rdf:type rdf:resource="&swrl;Variable"/>
    </rdf:Description>
    <rdf:Description rdf:about="urn:swrl#measure">
        <rdf:type rdf:resource="&swrl;Variable"/>
    </rdf:Description>
    <rdf:Description rdf:about="urn:swrl#measure3">
        <rdf:type rdf:resource="&swrl;Variable"/>
    </rdf:Description>
    <rdf:Description rdf:about="urn:swrl#individual3">
        <rdf:type rdf:resource="&swrl;Variable"/>
    </rdf:Description>
    <rdf:Description rdf:about="urn:swrl#value3">
        <rdf:type rdf:resource="&swrl;Variable"/>
    </rdf:Description>
    <rdf:Description rdf:about="urn:swrl#value4">
        <rdf:type rdf:resource="&swrl;Variable"/>
    </rdf:Description>
    <rdf:Description rdf:about="urn:swrl#value1">
        <rdf:type rdf:resource="&swrl;Variable"/>
    </rdf:Description>
    <rdf:Description rdf:about="urn:swrl#value2">
        <rdf:type rdf:resource="&swrl;Variable"/>
    </rdf:Description>
    <rdf:Description rdf:about="urn:swrl#literal3">
        <rdf:type rdf:resource="&swrl;Variable"/>
    </rdf:Description>
    <rdf:Description>
        <rdf:type rdf:resource="&swrl;Imp"/>
        <swrl:head>
            <rdf:Description>
                <rdf:type rdf:resource="&swrl;AtomList"/>
                <rdf:rest rdf:resource="&rdf;nil"/>
                <rdf:first>
                    <rdf:Description>
                        <rdf:type rdf:resource="&swrl;SameIndividualAtom"/>
                        <swrl:argument1 rdf:resource="urn:swrl#individual1"/>
                        <swrl:argument2 rdf:resource="urn:swrl#individual2"/>
                    </rdf:Description>
                </rdf:first>
            </rdf:Description>
        </swrl:head>
        <swrl:body>
            <rdf:Description>
                <rdf:type rdf:resource="&swrl;AtomList"/>
                <rdf:first>
                    <rdf:Description>
                        <rdf:type rdf:resource="&swrl;ClassAtom"/>
                        <swrl:classPredicate rdf:resource="http://purl.org/ceu/simeon#DistanceMeasure"/>
                        <swrl:argument1 rdf:resource="urn:swrl#measure"/>
                    </rdf:Description>
                </rdf:first>
                <rdf:rest>
                    <rdf:Description>
                        <rdf:type rdf:resource="&swrl;AtomList"/>
                        <rdf:first>
                            <rdf:Description>
                                <rdf:type rdf:resource="&swrl;IndividualPropertyAtom"/>
                                <swrl:propertyPredicate rdf:resource="http://purl.org/ceu/simeon#hasSourceObject"/>
                                <swrl:argument2 rdf:resource="urn:swrl#individual1"/>
                                <swrl:argument1 rdf:resource="urn:swrl#measure"/>
                            </rdf:Description>
                        </rdf:first>
                        <rdf:rest>
                            <rdf:Description>
                                <rdf:type rdf:resource="&swrl;AtomList"/>
                                <rdf:first>
                                    <rdf:Description>
                                        <rdf:type rdf:resource="&swrl;IndividualPropertyAtom"/>
                                        <swrl:propertyPredicate rdf:resource="http://purl.org/ceu/simeon#hasTargetObject"/>
                                        <swrl:argument2 rdf:resource="urn:swrl#individual2"/>
                                        <swrl:argument1 rdf:resource="urn:swrl#measure"/>
                                    </rdf:Description>
                                </rdf:first>
                                <rdf:rest>
                                    <rdf:Description>
                                        <rdf:type rdf:resource="&swrl;AtomList"/>
                                        <rdf:rest rdf:resource="&rdf;nil"/>
                                        <rdf:first>
                                            <rdf:Description>
                                                <rdf:type rdf:resource="&swrl;DatavaluedPropertyAtom"/>
                                                <swrl:argument2 rdf:datatype="&xsd;integer">0</swrl:argument2>
                                                <swrl:propertyPredicate rdf:resource="http://purl.org/ceu/simeon#hasValue"/>
                                                <swrl:argument1 rdf:resource="urn:swrl#measure"/>
                                            </rdf:Description>
                                        </rdf:first>
                                    </rdf:Description>
                                </rdf:rest>
                            </rdf:Description>
                        </rdf:rest>
                    </rdf:Description>
                </rdf:rest>
            </rdf:Description>
        </swrl:body>
    </rdf:Description>
    <rdf:Description>
        <rdf:type rdf:resource="&swrl;Imp"/>
        <swrl:body>
            <rdf:Description>
                <rdf:type rdf:resource="&swrl;AtomList"/>
                <rdf:first>
                    <rdf:Description>
                        <rdf:type rdf:resource="&swrl;ClassAtom"/>
                        <swrl:classPredicate rdf:resource="http://purl.org/ceu/simeon#DistanceMeasure"/>
                        <swrl:argument1 rdf:resource="urn:swrl#measure1"/>
                    </rdf:Description>
                </rdf:first>
                <rdf:rest>
                    <rdf:Description>
                        <rdf:type rdf:resource="&swrl;AtomList"/>
                        <rdf:rest>
                            <rdf:Description>
                                <rdf:type rdf:resource="&swrl;AtomList"/>
                                <rdf:rest>
                                    <rdf:Description>
                                        <rdf:type rdf:resource="&swrl;AtomList"/>
                                        <rdf:rest>
                                            <rdf:Description>
                                                <rdf:type rdf:resource="&swrl;AtomList"/>
                                                <rdf:first>
                                                    <rdf:Description>
                                                        <rdf:type rdf:resource="&swrl;IndividualPropertyAtom"/>
                                                        <swrl:propertyPredicate rdf:resource="http://purl.org/ceu/simeon#hasTargetObject"/>
                                                        <swrl:argument2 rdf:resource="urn:swrl#individual3"/>
                                                        <swrl:argument1 rdf:resource="urn:swrl#measure2"/>
                                                    </rdf:Description>
                                                </rdf:first>
                                                <rdf:rest>
                                                    <rdf:Description>
                                                        <rdf:type rdf:resource="&swrl;AtomList"/>
                                                        <rdf:first>
                                                            <rdf:Description>
                                                                <rdf:type rdf:resource="&swrl;IndividualPropertyAtom"/>
                                                                <swrl:propertyPredicate rdf:resource="http://purl.org/ceu/simeon#hasSourceObject"/>
                                                                <swrl:argument2 rdf:resource="urn:swrl#individual1"/>
                                                                <swrl:argument1 rdf:resource="urn:swrl#measure1"/>
                                                            </rdf:Description>
                                                        </rdf:first>
                                                        <rdf:rest>
                                                            <rdf:Description>
                                                                <rdf:type rdf:resource="&swrl;AtomList"/>
                                                                <rdf:rest>
                                                                    <rdf:Description>
                                                                        <rdf:type rdf:resource="&swrl;AtomList"/>
                                                                        <rdf:rest>
                                                                            <rdf:Description>
                                                                                <rdf:type rdf:resource="&swrl;AtomList"/>
                                                                                <rdf:first>
                                                                                    <rdf:Description>
                                                                                        <rdf:type rdf:resource="&swrl;DatavaluedPropertyAtom"/>
                                                                                        <swrl:propertyPredicate rdf:resource="http://purl.org/ceu/simeon#hasValue"/>
                                                                                        <swrl:argument1 rdf:resource="urn:swrl#measure3"/>
                                                                                        <swrl:argument2 rdf:resource="urn:swrl#value3"/>
                                                                                    </rdf:Description>
                                                                                </rdf:first>
                                                                                <rdf:rest>
                                                                                    <rdf:Description>
                                                                                        <rdf:type rdf:resource="&swrl;AtomList"/>
                                                                                        <rdf:rest>
                                                                                            <rdf:Description>
                                                                                                <rdf:type rdf:resource="&swrl;AtomList"/>
                                                                                                <rdf:rest>
                                                                                                    <rdf:Description>
                                                                                                        <rdf:type rdf:resource="&swrl;AtomList"/>
                                                                                                        <rdf:rest>
                                                                                                            <rdf:Description>
                                                                                                                <rdf:type rdf:resource="&swrl;AtomList"/>
                                                                                                                <rdf:first>
                                                                                                                    <rdf:Description>
                                                                                                                        <rdf:type rdf:resource="&swrl;IndividualPropertyAtom"/>
                                                                                                                        <swrl:propertyPredicate rdf:resource="http://purl.org/ceu/simeon#hasSourceObject"/>
                                                                                                                        <swrl:argument2 rdf:resource="urn:swrl#individual1"/>
                                                                                                                        <swrl:argument1 rdf:resource="urn:swrl#measure3"/>
                                                                                                                    </rdf:Description>
                                                                                                                </rdf:first>
                                                                                                                <rdf:rest>
                                                                                                                    <rdf:Description>
                                                                                                                        <rdf:type rdf:resource="&swrl;AtomList"/>
                                                                                                                        <rdf:first>
                                                                                                                            <rdf:Description>
                                                                                                                                <rdf:type rdf:resource="&swrl;DatavaluedPropertyAtom"/>
                                                                                                                                <swrl:propertyPredicate rdf:resource="http://purl.org/ceu/simeon#hasValue"/>
                                                                                                                                <swrl:argument1 rdf:resource="urn:swrl#measure2"/>
                                                                                                                                <swrl:argument2 rdf:resource="urn:swrl#value2"/>
                                                                                                                            </rdf:Description>
                                                                                                                        </rdf:first>
                                                                                                                        <rdf:rest>
                                                                                                                            <rdf:Description>
                                                                                                                                <rdf:type rdf:resource="&swrl;AtomList"/>
                                                                                                                                <rdf:rest>
                                                                                                                                    <rdf:Description>
                                                                                                                                        <rdf:type rdf:resource="&swrl;AtomList"/>
                                                                                                                                        <rdf:rest rdf:resource="&rdf;nil"/>
                                                                                                                                        <rdf:first>
                                                                                                                                            <rdf:Description>
                                                                                                                                                <rdf:type rdf:resource="&swrl;DatavaluedPropertyAtom"/>
                                                                                                                                                <swrl:propertyPredicate rdf:resource="http://purl.org/ceu/simeon#hasValue"/>
                                                                                                                                                <swrl:argument1 rdf:resource="urn:swrl#measure1"/>
                                                                                                                                                <swrl:argument2 rdf:resource="urn:swrl#value1"/>
                                                                                                                                            </rdf:Description>
                                                                                                                                        </rdf:first>
                                                                                                                                    </rdf:Description>
                                                                                                                                </rdf:rest>
                                                                                                                                <rdf:first>
                                                                                                                                    <rdf:Description>
                                                                                                                                        <rdf:type rdf:resource="&swrl;ClassAtom"/>
                                                                                                                                        <swrl:classPredicate rdf:resource="http://purl.org/ceu/simeon#DistanceMeasure"/>
                                                                                                                                        <swrl:argument1 rdf:resource="urn:swrl#measure2"/>
                                                                                                                                    </rdf:Description>
                                                                                                                                </rdf:first>
                                                                                                                            </rdf:Description>
                                                                                                                        </rdf:rest>
                                                                                                                    </rdf:Description>
                                                                                                                </rdf:rest>
                                                                                                            </rdf:Description>
                                                                                                        </rdf:rest>
                                                                                                        <rdf:first>
                                                                                                            <rdf:Description>
                                                                                                                <rdf:type rdf:resource="&swrl;IndividualPropertyAtom"/>
                                                                                                                <swrl:propertyPredicate rdf:resource="http://purl.org/ceu/simeon#usesComparisonMethod"/>
                                                                                                                <swrl:argument1 rdf:resource="urn:swrl#measure1"/>
                                                                                                                <swrl:argument2 rdf:resource="urn:swrl#method"/>
                                                                                                            </rdf:Description>
                                                                                                        </rdf:first>
                                                                                                    </rdf:Description>
                                                                                                </rdf:rest>
                                                                                                <rdf:first>
                                                                                                    <rdf:Description>
                                                                                                        <rdf:type rdf:resource="&swrl;ClassAtom"/>
                                                                                                        <swrl:classPredicate rdf:resource="http://purl.org/ceu/simeon#DistanceMeasure"/>
                                                                                                        <swrl:argument1 rdf:resource="urn:swrl#measure3"/>
                                                                                                    </rdf:Description>
                                                                                                </rdf:first>
                                                                                            </rdf:Description>
                                                                                        </rdf:rest>
                                                                                        <rdf:first>
                                                                                            <rdf:Description>
                                                                                                <rdf:type rdf:resource="&swrl;BuiltinAtom"/>
                                                                                                <swrl:builtin rdf:resource="&swrlb;add"/>
                                                                                                <swrl:arguments rdf:parseType="Collection">
                                                                                                    <rdf:Description rdf:about="urn:swrl#value4"/>
                                                                                                    <rdf:Description rdf:about="urn:swrl#value1"/>
                                                                                                    <rdf:Description rdf:about="urn:swrl#value2"/>
                                                                                                </swrl:arguments>
                                                                                            </rdf:Description>
                                                                                        </rdf:first>
                                                                                    </rdf:Description>
                                                                                </rdf:rest>
                                                                            </rdf:Description>
                                                                        </rdf:rest>
                                                                        <rdf:first>
                                                                            <rdf:Description>
                                                                                <rdf:type rdf:resource="&swrl;IndividualPropertyAtom"/>
                                                                                <swrl:propertyPredicate rdf:resource="http://purl.org/ceu/simeon#hasSourceObject"/>
                                                                                <swrl:argument2 rdf:resource="urn:swrl#individual2"/>
                                                                                <swrl:argument1 rdf:resource="urn:swrl#measure2"/>
                                                                            </rdf:Description>
                                                                        </rdf:first>
                                                                    </rdf:Description>
                                                                </rdf:rest>
                                                                <rdf:first>
                                                                    <rdf:Description>
                                                                        <rdf:type rdf:resource="&swrl;IndividualPropertyAtom"/>
                                                                        <swrl:propertyPredicate rdf:resource="http://purl.org/ceu/simeon#hasTargetObject"/>
                                                                        <swrl:argument2 rdf:resource="urn:swrl#individual2"/>
                                                                        <swrl:argument1 rdf:resource="urn:swrl#measure1"/>
                                                                    </rdf:Description>
                                                                </rdf:first>
                                                            </rdf:Description>
                                                        </rdf:rest>
                                                    </rdf:Description>
                                                </rdf:rest>
                                            </rdf:Description>
                                        </rdf:rest>
                                        <rdf:first>
                                            <rdf:Description>
                                                <rdf:type rdf:resource="&swrl;IndividualPropertyAtom"/>
                                                <swrl:propertyPredicate rdf:resource="http://purl.org/ceu/simeon#usesComparisonMethod"/>
                                                <swrl:argument1 rdf:resource="urn:swrl#measure3"/>
                                                <swrl:argument2 rdf:resource="urn:swrl#method"/>
                                            </rdf:Description>
                                        </rdf:first>
                                    </rdf:Description>
                                </rdf:rest>
                                <rdf:first>
                                    <rdf:Description>
                                        <rdf:type rdf:resource="&swrl;IndividualPropertyAtom"/>
                                        <swrl:propertyPredicate rdf:resource="http://purl.org/ceu/simeon#hasTargetObject"/>
                                        <swrl:argument2 rdf:resource="urn:swrl#individual3"/>
                                        <swrl:argument1 rdf:resource="urn:swrl#measure3"/>
                                    </rdf:Description>
                                </rdf:first>
                            </rdf:Description>
                        </rdf:rest>
                        <rdf:first>
                            <rdf:Description>
                                <rdf:type rdf:resource="&swrl;IndividualPropertyAtom"/>
                                <swrl:propertyPredicate rdf:resource="http://purl.org/ceu/simeon#usesComparisonMethod"/>
                                <swrl:argument1 rdf:resource="urn:swrl#measure2"/>
                                <swrl:argument2 rdf:resource="urn:swrl#method"/>
                            </rdf:Description>
                        </rdf:first>
                    </rdf:Description>
                </rdf:rest>
            </rdf:Description>
        </swrl:body>
        <swrl:head>
            <rdf:Description>
                <rdf:type rdf:resource="&swrl;AtomList"/>
                <rdf:rest rdf:resource="&rdf;nil"/>
                <rdf:first>
                    <rdf:Description>
                        <rdf:type rdf:resource="&swrl;BuiltinAtom"/>
                        <swrl:builtin rdf:resource="&swrlb;greaterThanOrEqual"/>
                        <swrl:arguments rdf:parseType="Collection">
                            <rdf:Description rdf:about="urn:swrl#value4"/>
                            <rdf:Description rdf:about="urn:swrl#value3"/>
                        </swrl:arguments>
                    </rdf:Description>
                </rdf:first>
            </rdf:Description>
        </swrl:head>
    </rdf:Description>
    <rdf:Description>
        <rdf:type rdf:resource="&swrl;Imp"/>
        <swrl:head>
            <rdf:Description>
                <rdf:type rdf:resource="&swrl;AtomList"/>
                <rdf:rest rdf:resource="&rdf;nil"/>
                <rdf:first>
                    <rdf:Description>
                        <rdf:type rdf:resource="&swrl;DatavaluedPropertyAtom"/>
                        <swrl:argument2 rdf:datatype="&xsd;integer">0</swrl:argument2>
                        <swrl:propertyPredicate rdf:resource="http://purl.org/ceu/simeon#hasValue"/>
                        <swrl:argument1 rdf:resource="urn:swrl#measure"/>
                    </rdf:Description>
                </rdf:first>
            </rdf:Description>
        </swrl:head>
        <swrl:body>
            <rdf:Description>
                <rdf:type rdf:resource="&swrl;AtomList"/>
                <rdf:first>
                    <rdf:Description>
                        <rdf:type rdf:resource="&swrl;IndividualPropertyAtom"/>
                        <swrl:argument2 rdf:resource="http://purl.org/ceu/simeon#objectIdentitySimilarityFunction"/>
                        <swrl:propertyPredicate rdf:resource="http://purl.org/ceu/simeon#usesComparisonMethod"/>
                        <swrl:argument1 rdf:resource="urn:swrl#measure"/>
                    </rdf:Description>
                </rdf:first>
                <rdf:rest>
                    <rdf:Description>
                        <rdf:type rdf:resource="&swrl;AtomList"/>
                        <rdf:rest>
                            <rdf:Description>
                                <rdf:type rdf:resource="&swrl;AtomList"/>
                                <rdf:rest>
                                    <rdf:Description>
                                        <rdf:type rdf:resource="&swrl;AtomList"/>
                                        <rdf:rest>
                                            <rdf:Description>
                                                <rdf:type rdf:resource="&swrl;AtomList"/>
                                                <rdf:rest rdf:resource="&rdf;nil"/>
                                                <rdf:first>
                                                    <rdf:Description>
                                                        <rdf:type rdf:resource="&swrl;DifferentIndividualsAtom"/>
                                                        <swrl:argument1 rdf:resource="urn:swrl#individual1"/>
                                                        <swrl:argument2 rdf:resource="urn:swrl#individual2"/>
                                                    </rdf:Description>
                                                </rdf:first>
                                            </rdf:Description>
                                        </rdf:rest>
                                        <rdf:first>
                                            <rdf:Description>
                                                <rdf:type rdf:resource="&swrl;ClassAtom"/>
                                                <swrl:classPredicate rdf:resource="http://purl.org/ceu/simeon#SimilarityMeasure"/>
                                                <swrl:argument1 rdf:resource="urn:swrl#measure"/>
                                            </rdf:Description>
                                        </rdf:first>
                                    </rdf:Description>
                                </rdf:rest>
                                <rdf:first>
                                    <rdf:Description>
                                        <rdf:type rdf:resource="&swrl;IndividualPropertyAtom"/>
                                        <swrl:propertyPredicate rdf:resource="http://purl.org/ceu/simeon#hasTargetObject"/>
                                        <swrl:argument2 rdf:resource="urn:swrl#individual2"/>
                                        <swrl:argument1 rdf:resource="urn:swrl#measure"/>
                                    </rdf:Description>
                                </rdf:first>
                            </rdf:Description>
                        </rdf:rest>
                        <rdf:first>
                            <rdf:Description>
                                <rdf:type rdf:resource="&swrl;IndividualPropertyAtom"/>
                                <swrl:propertyPredicate rdf:resource="http://purl.org/ceu/simeon#hasSourceObject"/>
                                <swrl:argument2 rdf:resource="urn:swrl#individual1"/>
                                <swrl:argument1 rdf:resource="urn:swrl#measure"/>
                            </rdf:Description>
                        </rdf:first>
                    </rdf:Description>
                </rdf:rest>
            </rdf:Description>
        </swrl:body>
    </rdf:Description>
    <rdf:Description>
        <rdf:type rdf:resource="&swrl;Imp"/>
        <swrl:head>
            <rdf:Description>
                <rdf:type rdf:resource="&swrl;AtomList"/>
                <rdf:rest rdf:resource="&rdf;nil"/>
                <rdf:first>
                    <rdf:Description>
                        <rdf:type rdf:resource="&swrl;SameIndividualAtom"/>
                        <swrl:argument1 rdf:resource="urn:swrl#literal1"/>
                        <swrl:argument2 rdf:resource="urn:swrl#literal2"/>
                    </rdf:Description>
                </rdf:first>
            </rdf:Description>
        </swrl:head>
        <swrl:body>
            <rdf:Description>
                <rdf:type rdf:resource="&swrl;AtomList"/>
                <rdf:first>
                    <rdf:Description>
                        <rdf:type rdf:resource="&swrl;ClassAtom"/>
                        <swrl:classPredicate rdf:resource="http://purl.org/ceu/simeon#DistanceMeasure"/>
                        <swrl:argument1 rdf:resource="urn:swrl#measure"/>
                    </rdf:Description>
                </rdf:first>
                <rdf:rest>
                    <rdf:Description>
                        <rdf:type rdf:resource="&swrl;AtomList"/>
                        <rdf:first>
                            <rdf:Description>
                                <rdf:type rdf:resource="&swrl;DatavaluedPropertyAtom"/>
                                <swrl:propertyPredicate rdf:resource="http://purl.org/ceu/simeon#hasTargetData"/>
                                <swrl:argument2 rdf:resource="urn:swrl#literal2"/>
                                <swrl:argument1 rdf:resource="urn:swrl#measure"/>
                            </rdf:Description>
                        </rdf:first>
                        <rdf:rest>
                            <rdf:Description>
                                <rdf:type rdf:resource="&swrl;AtomList"/>
                                <rdf:rest>
                                    <rdf:Description>
                                        <rdf:type rdf:resource="&swrl;AtomList"/>
                                        <rdf:rest rdf:resource="&rdf;nil"/>
                                        <rdf:first>
                                            <rdf:Description>
                                                <rdf:type rdf:resource="&swrl;DatavaluedPropertyAtom"/>
                                                <swrl:propertyPredicate rdf:resource="http://purl.org/ceu/simeon#hasSourceData"/>
                                                <swrl:argument2 rdf:resource="urn:swrl#literal1"/>
                                                <swrl:argument1 rdf:resource="urn:swrl#measure"/>
                                            </rdf:Description>
                                        </rdf:first>
                                    </rdf:Description>
                                </rdf:rest>
                                <rdf:first>
                                    <rdf:Description>
                                        <rdf:type rdf:resource="&swrl;DatavaluedPropertyAtom"/>
                                        <swrl:argument2 rdf:datatype="&xsd;integer">0</swrl:argument2>
                                        <swrl:propertyPredicate rdf:resource="http://purl.org/ceu/simeon#hasValue"/>
                                        <swrl:argument1 rdf:resource="urn:swrl#measure"/>
                                    </rdf:Description>
                                </rdf:first>
                            </rdf:Description>
                        </rdf:rest>
                    </rdf:Description>
                </rdf:rest>
            </rdf:Description>
        </swrl:body>
    </rdf:Description>
    <rdf:Description>
        <rdf:type rdf:resource="&swrl;Imp"/>
        <swrl:body>
            <rdf:Description>
                <rdf:type rdf:resource="&swrl;AtomList"/>
                <rdf:first>
                    <rdf:Description>
                        <rdf:type rdf:resource="&swrl;ClassAtom"/>
                        <swrl:classPredicate rdf:resource="http://purl.org/ceu/simeon#DistanceMeasure"/>
                        <swrl:argument1 rdf:resource="urn:swrl#measure1"/>
                    </rdf:Description>
                </rdf:first>
                <rdf:rest>
                    <rdf:Description>
                        <rdf:type rdf:resource="&swrl;AtomList"/>
                        <rdf:rest>
                            <rdf:Description>
                                <rdf:type rdf:resource="&swrl;AtomList"/>
                                <rdf:rest>
                                    <rdf:Description>
                                        <rdf:type rdf:resource="&swrl;AtomList"/>
                                        <rdf:first>
                                            <rdf:Description>
                                                <rdf:type rdf:resource="&swrl;DatavaluedPropertyAtom"/>
                                                <swrl:propertyPredicate rdf:resource="http://purl.org/ceu/simeon#hasTargetData"/>
                                                <swrl:argument2 rdf:resource="urn:swrl#literal3"/>
                                                <swrl:argument1 rdf:resource="urn:swrl#measure3"/>
                                            </rdf:Description>
                                        </rdf:first>
                                        <rdf:rest>
                                            <rdf:Description>
                                                <rdf:type rdf:resource="&swrl;AtomList"/>
                                                <rdf:rest>
                                                    <rdf:Description>
                                                        <rdf:type rdf:resource="&swrl;AtomList"/>
                                                        <rdf:first>
                                                            <rdf:Description>
                                                                <rdf:type rdf:resource="&swrl;DatavaluedPropertyAtom"/>
                                                                <swrl:propertyPredicate rdf:resource="http://purl.org/ceu/simeon#hasSourceData"/>
                                                                <swrl:argument2 rdf:resource="urn:swrl#literal2"/>
                                                                <swrl:argument1 rdf:resource="urn:swrl#measure2"/>
                                                            </rdf:Description>
                                                        </rdf:first>
                                                        <rdf:rest>
                                                            <rdf:Description>
                                                                <rdf:type rdf:resource="&swrl;AtomList"/>
                                                                <rdf:first>
                                                                    <rdf:Description>
                                                                        <rdf:type rdf:resource="&swrl;DatavaluedPropertyAtom"/>
                                                                        <swrl:propertyPredicate rdf:resource="http://purl.org/ceu/simeon#hasValue"/>
                                                                        <swrl:argument1 rdf:resource="urn:swrl#measure3"/>
                                                                        <swrl:argument2 rdf:resource="urn:swrl#value3"/>
                                                                    </rdf:Description>
                                                                </rdf:first>
                                                                <rdf:rest>
                                                                    <rdf:Description>
                                                                        <rdf:type rdf:resource="&swrl;AtomList"/>
                                                                        <rdf:first>
                                                                            <rdf:Description>
                                                                                <rdf:type rdf:resource="&swrl;BuiltinAtom"/>
                                                                                <swrl:builtin rdf:resource="&swrlb;add"/>
                                                                                <swrl:arguments rdf:parseType="Collection">
                                                                                    <rdf:Description rdf:about="urn:swrl#value4"/>
                                                                                    <rdf:Description rdf:about="urn:swrl#value1"/>
                                                                                    <rdf:Description rdf:about="urn:swrl#value2"/>
                                                                                </swrl:arguments>
                                                                            </rdf:Description>
                                                                        </rdf:first>
                                                                        <rdf:rest>
                                                                            <rdf:Description>
                                                                                <rdf:type rdf:resource="&swrl;AtomList"/>
                                                                                <rdf:first>
                                                                                    <rdf:Description>
                                                                                        <rdf:type rdf:resource="&swrl;DatavaluedPropertyAtom"/>
                                                                                        <swrl:propertyPredicate rdf:resource="http://purl.org/ceu/simeon#hasSourceData"/>
                                                                                        <swrl:argument2 rdf:resource="urn:swrl#literal1"/>
                                                                                        <swrl:argument1 rdf:resource="urn:swrl#measure1"/>
                                                                                    </rdf:Description>
                                                                                </rdf:first>
                                                                                <rdf:rest>
                                                                                    <rdf:Description>
                                                                                        <rdf:type rdf:resource="&swrl;AtomList"/>
                                                                                        <rdf:rest>
                                                                                            <rdf:Description>
                                                                                                <rdf:type rdf:resource="&swrl;AtomList"/>
                                                                                                <rdf:rest>
                                                                                                    <rdf:Description>
                                                                                                        <rdf:type rdf:resource="&swrl;AtomList"/>
                                                                                                        <rdf:rest>
                                                                                                            <rdf:Description>
                                                                                                                <rdf:type rdf:resource="&swrl;AtomList"/>
                                                                                                                <rdf:rest>
                                                                                                                    <rdf:Description>
                                                                                                                        <rdf:type rdf:resource="&swrl;AtomList"/>
                                                                                                                        <rdf:first>
                                                                                                                            <rdf:Description>
                                                                                                                                <rdf:type rdf:resource="&swrl;ClassAtom"/>
                                                                                                                                <swrl:classPredicate rdf:resource="http://purl.org/ceu/simeon#DistanceMeasure"/>
                                                                                                                                <swrl:argument1 rdf:resource="urn:swrl#measure2"/>
                                                                                                                            </rdf:Description>
                                                                                                                        </rdf:first>
                                                                                                                        <rdf:rest>
                                                                                                                            <rdf:Description>
                                                                                                                                <rdf:type rdf:resource="&swrl;AtomList"/>
                                                                                                                                <rdf:first>
                                                                                                                                    <rdf:Description>
                                                                                                                                        <rdf:type rdf:resource="&swrl;DatavaluedPropertyAtom"/>
                                                                                                                                        <swrl:propertyPredicate rdf:resource="http://purl.org/ceu/simeon#hasValue"/>
                                                                                                                                        <swrl:argument1 rdf:resource="urn:swrl#measure1"/>
                                                                                                                                        <swrl:argument2 rdf:resource="urn:swrl#value1"/>
                                                                                                                                    </rdf:Description>
                                                                                                                                </rdf:first>
                                                                                                                                <rdf:rest>
                                                                                                                                    <rdf:Description>
                                                                                                                                        <rdf:type rdf:resource="&swrl;AtomList"/>
                                                                                                                                        <rdf:rest rdf:resource="&rdf;nil"/>
                                                                                                                                        <rdf:first>
                                                                                                                                            <rdf:Description>
                                                                                                                                                <rdf:type rdf:resource="&swrl;DatavaluedPropertyAtom"/>
                                                                                                                                                <swrl:propertyPredicate rdf:resource="http://purl.org/ceu/simeon#hasTargetData"/>
                                                                                                                                                <swrl:argument2 rdf:resource="urn:swrl#literal3"/>
                                                                                                                                                <swrl:argument1 rdf:resource="urn:swrl#measure2"/>
                                                                                                                                            </rdf:Description>
                                                                                                                                        </rdf:first>
                                                                                                                                    </rdf:Description>
                                                                                                                                </rdf:rest>
                                                                                                                            </rdf:Description>
                                                                                                                        </rdf:rest>
                                                                                                                    </rdf:Description>
                                                                                                                </rdf:rest>
                                                                                                                <rdf:first>
                                                                                                                    <rdf:Description>
                                                                                                                        <rdf:type rdf:resource="&swrl;DatavaluedPropertyAtom"/>
                                                                                                                        <swrl:propertyPredicate rdf:resource="http://purl.org/ceu/simeon#hasValue"/>
                                                                                                                        <swrl:argument1 rdf:resource="urn:swrl#measure2"/>
                                                                                                                        <swrl:argument2 rdf:resource="urn:swrl#value2"/>
                                                                                                                    </rdf:Description>
                                                                                                                </rdf:first>
                                                                                                            </rdf:Description>
                                                                                                        </rdf:rest>
                                                                                                        <rdf:first>
                                                                                                            <rdf:Description>
                                                                                                                <rdf:type rdf:resource="&swrl;DatavaluedPropertyAtom"/>
                                                                                                                <swrl:propertyPredicate rdf:resource="http://purl.org/ceu/simeon#hasTargetData"/>
                                                                                                                <swrl:argument2 rdf:resource="urn:swrl#literal2"/>
                                                                                                                <swrl:argument1 rdf:resource="urn:swrl#measure1"/>
                                                                                                            </rdf:Description>
                                                                                                        </rdf:first>
                                                                                                    </rdf:Description>
                                                                                                </rdf:rest>
                                                                                                <rdf:first>
                                                                                                    <rdf:Description>
                                                                                                        <rdf:type rdf:resource="&swrl;IndividualPropertyAtom"/>
                                                                                                        <swrl:propertyPredicate rdf:resource="http://purl.org/ceu/simeon#usesComparisonMethod"/>
                                                                                                        <swrl:argument1 rdf:resource="urn:swrl#measure1"/>
                                                                                                        <swrl:argument2 rdf:resource="urn:swrl#method"/>
                                                                                                    </rdf:Description>
                                                                                                </rdf:first>
                                                                                            </rdf:Description>
                                                                                        </rdf:rest>
                                                                                        <rdf:first>
                                                                                            <rdf:Description>
                                                                                                <rdf:type rdf:resource="&swrl;ClassAtom"/>
                                                                                                <swrl:classPredicate rdf:resource="http://purl.org/ceu/simeon#DistanceMeasure"/>
                                                                                                <swrl:argument1 rdf:resource="urn:swrl#measure3"/>
                                                                                            </rdf:Description>
                                                                                        </rdf:first>
                                                                                    </rdf:Description>
                                                                                </rdf:rest>
                                                                            </rdf:Description>
                                                                        </rdf:rest>
                                                                    </rdf:Description>
                                                                </rdf:rest>
                                                            </rdf:Description>
                                                        </rdf:rest>
                                                    </rdf:Description>
                                                </rdf:rest>
                                                <rdf:first>
                                                    <rdf:Description>
                                                        <rdf:type rdf:resource="&swrl;IndividualPropertyAtom"/>
                                                        <swrl:propertyPredicate rdf:resource="http://purl.org/ceu/simeon#usesComparisonMethod"/>
                                                        <swrl:argument1 rdf:resource="urn:swrl#measure3"/>
                                                        <swrl:argument2 rdf:resource="urn:swrl#method"/>
                                                    </rdf:Description>
                                                </rdf:first>
                                            </rdf:Description>
                                        </rdf:rest>
                                    </rdf:Description>
                                </rdf:rest>
                                <rdf:first>
                                    <rdf:Description>
                                        <rdf:type rdf:resource="&swrl;DatavaluedPropertyAtom"/>
                                        <swrl:propertyPredicate rdf:resource="http://purl.org/ceu/simeon#hasSourceData"/>
                                        <swrl:argument2 rdf:resource="urn:swrl#literal1"/>
                                        <swrl:argument1 rdf:resource="urn:swrl#measure3"/>
                                    </rdf:Description>
                                </rdf:first>
                            </rdf:Description>
                        </rdf:rest>
                        <rdf:first>
                            <rdf:Description>
                                <rdf:type rdf:resource="&swrl;IndividualPropertyAtom"/>
                                <swrl:propertyPredicate rdf:resource="http://purl.org/ceu/simeon#usesComparisonMethod"/>
                                <swrl:argument1 rdf:resource="urn:swrl#measure2"/>
                                <swrl:argument2 rdf:resource="urn:swrl#method"/>
                            </rdf:Description>
                        </rdf:first>
                    </rdf:Description>
                </rdf:rest>
            </rdf:Description>
        </swrl:body>
        <swrl:head>
            <rdf:Description>
                <rdf:type rdf:resource="&swrl;AtomList"/>
                <rdf:rest rdf:resource="&rdf;nil"/>
                <rdf:first>
                    <rdf:Description>
                        <rdf:type rdf:resource="&swrl;BuiltinAtom"/>
                        <swrl:builtin rdf:resource="&swrlb;greaterThanOrEqual"/>
                        <swrl:arguments rdf:parseType="Collection">
                            <rdf:Description rdf:about="urn:swrl#value4"/>
                            <rdf:Description rdf:about="urn:swrl#value3"/>
                        </swrl:arguments>
                    </rdf:Description>
                </rdf:first>
            </rdf:Description>
        </swrl:head>
    </rdf:Description>
    <rdf:Description>
        <rdf:type rdf:resource="&swrl;Imp"/>
        <swrl:head>
            <rdf:Description>
                <rdf:type rdf:resource="&swrl;AtomList"/>
                <rdf:first>
                    <rdf:Description>
                        <rdf:type rdf:resource="&swrl;DatavaluedPropertyAtom"/>
                        <swrl:propertyPredicate rdf:resource="http://purl.org/ceu/simeon#hasTargetData"/>
                        <swrl:argument2 rdf:resource="urn:swrl#literal1"/>
                        <swrl:argument1 rdf:resource="urn:swrl#measure2"/>
                    </rdf:Description>
                </rdf:first>
                <rdf:rest>
                    <rdf:Description>
                        <rdf:type rdf:resource="&swrl;AtomList"/>
                        <rdf:first>
                            <rdf:Description>
                                <rdf:type rdf:resource="&swrl;DatavaluedPropertyAtom"/>
                                <swrl:propertyPredicate rdf:resource="http://purl.org/ceu/simeon#hasSourceData"/>
                                <swrl:argument2 rdf:resource="urn:swrl#literal2"/>
                                <swrl:argument1 rdf:resource="urn:swrl#measure2"/>
                            </rdf:Description>
                        </rdf:first>
                        <rdf:rest>
                            <rdf:Description>
                                <rdf:type rdf:resource="&swrl;AtomList"/>
                                <rdf:first>
                                    <rdf:Description>
                                        <rdf:type rdf:resource="&swrl;ClassAtom"/>
                                        <swrl:classPredicate rdf:resource="http://purl.org/ceu/simeon#SymmetricComparisonMeasure"/>
                                        <swrl:argument1 rdf:resource="urn:swrl#measure2"/>
                                    </rdf:Description>
                                </rdf:first>
                                <rdf:rest>
                                    <rdf:Description>
                                        <rdf:type rdf:resource="&swrl;AtomList"/>
                                        <rdf:rest>
                                            <rdf:Description>
                                                <rdf:type rdf:resource="&swrl;AtomList"/>
                                                <rdf:rest rdf:resource="&rdf;nil"/>
                                                <rdf:first>
                                                    <rdf:Description>
                                                        <rdf:type rdf:resource="&swrl;DatavaluedPropertyAtom"/>
                                                        <swrl:propertyPredicate rdf:resource="http://purl.org/ceu/simeon#hasValue"/>
                                                        <swrl:argument1 rdf:resource="urn:swrl#measure2"/>
                                                        <swrl:argument2 rdf:resource="urn:swrl#value"/>
                                                    </rdf:Description>
                                                </rdf:first>
                                            </rdf:Description>
                                        </rdf:rest>
                                        <rdf:first>
                                            <rdf:Description>
                                                <rdf:type rdf:resource="&swrl;IndividualPropertyAtom"/>
                                                <swrl:propertyPredicate rdf:resource="http://purl.org/ceu/simeon#usesComparisonMethod"/>
                                                <swrl:argument1 rdf:resource="urn:swrl#measure2"/>
                                                <swrl:argument2 rdf:resource="urn:swrl#method"/>
                                            </rdf:Description>
                                        </rdf:first>
                                    </rdf:Description>
                                </rdf:rest>
                            </rdf:Description>
                        </rdf:rest>
                    </rdf:Description>
                </rdf:rest>
            </rdf:Description>
        </swrl:head>
        <swrl:body>
            <rdf:Description>
                <rdf:type rdf:resource="&swrl;AtomList"/>
                <rdf:rest>
                    <rdf:Description>
                        <rdf:type rdf:resource="&swrl;AtomList"/>
                        <rdf:rest>
                            <rdf:Description>
                                <rdf:type rdf:resource="&swrl;AtomList"/>
                                <rdf:first>
                                    <rdf:Description>
                                        <rdf:type rdf:resource="&swrl;IndividualPropertyAtom"/>
                                        <swrl:propertyPredicate rdf:resource="http://purl.org/ceu/simeon#usesComparisonMethod"/>
                                        <swrl:argument1 rdf:resource="urn:swrl#measure1"/>
                                        <swrl:argument2 rdf:resource="urn:swrl#method"/>
                                    </rdf:Description>
                                </rdf:first>
                                <rdf:rest>
                                    <rdf:Description>
                                        <rdf:type rdf:resource="&swrl;AtomList"/>
                                        <rdf:first>
                                            <rdf:Description>
                                                <rdf:type rdf:resource="&swrl;DatavaluedPropertyAtom"/>
                                                <swrl:propertyPredicate rdf:resource="http://purl.org/ceu/simeon#hasValue"/>
                                                <swrl:argument1 rdf:resource="urn:swrl#measure1"/>
                                                <swrl:argument2 rdf:resource="urn:swrl#value"/>
                                            </rdf:Description>
                                        </rdf:first>
                                        <rdf:rest>
                                            <rdf:Description>
                                                <rdf:type rdf:resource="&swrl;AtomList"/>
                                                <rdf:rest rdf:resource="&rdf;nil"/>
                                                <rdf:first>
                                                    <rdf:Description>
                                                        <rdf:type rdf:resource="&swrl;DatavaluedPropertyAtom"/>
                                                        <swrl:propertyPredicate rdf:resource="http://purl.org/ceu/simeon#hasTargetData"/>
                                                        <swrl:argument2 rdf:resource="urn:swrl#literal2"/>
                                                        <swrl:argument1 rdf:resource="urn:swrl#measure1"/>
                                                    </rdf:Description>
                                                </rdf:first>
                                            </rdf:Description>
                                        </rdf:rest>
                                    </rdf:Description>
                                </rdf:rest>
                            </rdf:Description>
                        </rdf:rest>
                        <rdf:first>
                            <rdf:Description>
                                <rdf:type rdf:resource="&swrl;DatavaluedPropertyAtom"/>
                                <swrl:propertyPredicate rdf:resource="http://purl.org/ceu/simeon#hasSourceData"/>
                                <swrl:argument2 rdf:resource="urn:swrl#literal1"/>
                                <swrl:argument1 rdf:resource="urn:swrl#measure1"/>
                            </rdf:Description>
                        </rdf:first>
                    </rdf:Description>
                </rdf:rest>
                <rdf:first>
                    <rdf:Description>
                        <rdf:type rdf:resource="&swrl;ClassAtom"/>
                        <swrl:classPredicate rdf:resource="http://purl.org/ceu/simeon#SymmetricComparisonMeasure"/>
                        <swrl:argument1 rdf:resource="urn:swrl#measure1"/>
                    </rdf:Description>
                </rdf:first>
            </rdf:Description>
        </swrl:body>
    </rdf:Description>
    <rdf:Description>
        <rdf:type rdf:resource="&swrl;Imp"/>
        <swrl:body>
            <rdf:Description>
                <rdf:type rdf:resource="&swrl;AtomList"/>
                <rdf:rest>
                    <rdf:Description>
                        <rdf:type rdf:resource="&swrl;AtomList"/>
                        <rdf:first>
                            <rdf:Description>
                                <rdf:type rdf:resource="&swrl;SameIndividualAtom"/>
                                <swrl:argument1 rdf:resource="urn:swrl#literal1"/>
                                <swrl:argument2 rdf:resource="urn:swrl#literal2"/>
                            </rdf:Description>
                        </rdf:first>
                        <rdf:rest>
                            <rdf:Description>
                                <rdf:type rdf:resource="&swrl;AtomList"/>
                                <rdf:first>
                                    <rdf:Description>
                                        <rdf:type rdf:resource="&swrl;ClassAtom"/>
                                        <swrl:classPredicate rdf:resource="http://purl.org/ceu/simeon#DissimilarityMeasure"/>
                                        <swrl:argument1 rdf:resource="urn:swrl#measure"/>
                                    </rdf:Description>
                                </rdf:first>
                                <rdf:rest>
                                    <rdf:Description>
                                        <rdf:type rdf:resource="&swrl;AtomList"/>
                                        <rdf:rest rdf:resource="&rdf;nil"/>
                                        <rdf:first>
                                            <rdf:Description>
                                                <rdf:type rdf:resource="&swrl;DatavaluedPropertyAtom"/>
                                                <swrl:propertyPredicate rdf:resource="http://purl.org/ceu/simeon#hasSourceData"/>
                                                <swrl:argument2 rdf:resource="urn:swrl#literal1"/>
                                                <swrl:argument1 rdf:resource="urn:swrl#measure"/>
                                            </rdf:Description>
                                        </rdf:first>
                                    </rdf:Description>
                                </rdf:rest>
                            </rdf:Description>
                        </rdf:rest>
                    </rdf:Description>
                </rdf:rest>
                <rdf:first>
                    <rdf:Description>
                        <rdf:type rdf:resource="&swrl;IndividualPropertyAtom"/>
                        <swrl:propertyPredicate rdf:resource="http://purl.org/ceu/simeon#hasTargetObject"/>
                        <swrl:argument2 rdf:resource="urn:swrl#literal2"/>
                        <swrl:argument1 rdf:resource="urn:swrl#measure"/>
                    </rdf:Description>
                </rdf:first>
            </rdf:Description>
        </swrl:body>
        <swrl:head>
            <rdf:Description>
                <rdf:type rdf:resource="&swrl;AtomList"/>
                <rdf:rest rdf:resource="&rdf;nil"/>
                <rdf:first>
                    <rdf:Description>
                        <rdf:type rdf:resource="&swrl;DatavaluedPropertyAtom"/>
                        <swrl:argument2 rdf:datatype="&xsd;integer">0</swrl:argument2>
                        <swrl:propertyPredicate rdf:resource="http://purl.org/ceu/simeon#hasValue"/>
                        <swrl:argument1 rdf:resource="urn:swrl#measure"/>
                    </rdf:Description>
                </rdf:first>
            </rdf:Description>
        </swrl:head>
    </rdf:Description>
    <rdf:Description>
        <rdf:type rdf:resource="&swrl;Imp"/>
        <swrl:head>
            <rdf:Description>
                <rdf:type rdf:resource="&swrl;AtomList"/>
                <rdf:rest rdf:resource="&rdf;nil"/>
                <rdf:first>
                    <rdf:Description>
                        <rdf:type rdf:resource="&swrl;BuiltinAtom"/>
                        <swrl:builtin rdf:resource="&swrlb;greaterThanOrEqual"/>
                        <swrl:arguments rdf:parseType="Collection">
                            <rdf:Description rdf:about="urn:swrl#value1"/>
                            <rdf:Description rdf:about="urn:swrl#value2"/>
                        </swrl:arguments>
                    </rdf:Description>
                </rdf:first>
            </rdf:Description>
        </swrl:head>
        <swrl:body>
            <rdf:Description>
                <rdf:type rdf:resource="&swrl;AtomList"/>
                <rdf:first>
                    <rdf:Description>
                        <rdf:type rdf:resource="&swrl;IndividualPropertyAtom"/>
                        <swrl:propertyPredicate rdf:resource="http://purl.org/ceu/simeon#hasSourceObject"/>
                        <swrl:argument2 rdf:resource="urn:swrl#individual1"/>
                        <swrl:argument1 rdf:resource="urn:swrl#measure2"/>
                    </rdf:Description>
                </rdf:first>
                <rdf:rest>
                    <rdf:Description>
                        <rdf:type rdf:resource="&swrl;AtomList"/>
                        <rdf:rest>
                            <rdf:Description>
                                <rdf:type rdf:resource="&swrl;AtomList"/>
                                <rdf:rest>
                                    <rdf:Description>
                                        <rdf:type rdf:resource="&swrl;AtomList"/>
                                        <rdf:first>
                                            <rdf:Description>
                                                <rdf:type rdf:resource="&swrl;IndividualPropertyAtom"/>
                                                <swrl:propertyPredicate rdf:resource="http://purl.org/ceu/simeon#hasTargetObject"/>
                                                <swrl:argument2 rdf:resource="urn:swrl#individual1"/>
                                                <swrl:argument1 rdf:resource="urn:swrl#measure1"/>
                                            </rdf:Description>
                                        </rdf:first>
                                        <rdf:rest>
                                            <rdf:Description>
                                                <rdf:type rdf:resource="&swrl;AtomList"/>
                                                <rdf:first>
                                                    <rdf:Description>
                                                        <rdf:type rdf:resource="&swrl;IndividualPropertyAtom"/>
                                                        <swrl:propertyPredicate rdf:resource="http://purl.org/ceu/simeon#usesComparisonMethod"/>
                                                        <swrl:argument1 rdf:resource="urn:swrl#measure1"/>
                                                        <swrl:argument2 rdf:resource="urn:swrl#method"/>
                                                    </rdf:Description>
                                                </rdf:first>
                                                <rdf:rest>
                                                    <rdf:Description>
                                                        <rdf:type rdf:resource="&swrl;AtomList"/>
                                                        <rdf:first>
                                                            <rdf:Description>
                                                                <rdf:type rdf:resource="&swrl;DatavaluedPropertyAtom"/>
                                                                <swrl:propertyPredicate rdf:resource="http://purl.org/ceu/simeon#hasValue"/>
                                                                <swrl:argument1 rdf:resource="urn:swrl#measure2"/>
                                                                <swrl:argument2 rdf:resource="urn:swrl#value2"/>
                                                            </rdf:Description>
                                                        </rdf:first>
                                                        <rdf:rest>
                                                            <rdf:Description>
                                                                <rdf:type rdf:resource="&swrl;AtomList"/>
                                                                <rdf:rest>
                                                                    <rdf:Description>
                                                                        <rdf:type rdf:resource="&swrl;AtomList"/>
                                                                        <rdf:first>
                                                                            <rdf:Description>
                                                                                <rdf:type rdf:resource="&swrl;IndividualPropertyAtom"/>
                                                                                <swrl:propertyPredicate rdf:resource="http://purl.org/ceu/simeon#hasSourceObject"/>
                                                                                <swrl:argument2 rdf:resource="urn:swrl#individual1"/>
                                                                                <swrl:argument1 rdf:resource="urn:swrl#measure1"/>
                                                                            </rdf:Description>
                                                                        </rdf:first>
                                                                        <rdf:rest>
                                                                            <rdf:Description>
                                                                                <rdf:type rdf:resource="&swrl;AtomList"/>
                                                                                <rdf:first>
                                                                                    <rdf:Description>
                                                                                        <rdf:type rdf:resource="&swrl;ClassAtom"/>
                                                                                        <swrl:classPredicate rdf:resource="http://purl.org/ceu/simeon#SimilarityMeasure"/>
                                                                                        <swrl:argument1 rdf:resource="urn:swrl#measure2"/>
                                                                                    </rdf:Description>
                                                                                </rdf:first>
                                                                                <rdf:rest>
                                                                                    <rdf:Description>
                                                                                        <rdf:type rdf:resource="&swrl;AtomList"/>
                                                                                        <rdf:rest>
                                                                                            <rdf:Description>
                                                                                                <rdf:type rdf:resource="&swrl;AtomList"/>
                                                                                                <rdf:rest rdf:resource="&rdf;nil"/>
                                                                                                <rdf:first>
                                                                                                    <rdf:Description>
                                                                                                        <rdf:type rdf:resource="&swrl;DatavaluedPropertyAtom"/>
                                                                                                        <swrl:propertyPredicate rdf:resource="http://purl.org/ceu/simeon#hasValue"/>
                                                                                                        <swrl:argument1 rdf:resource="urn:swrl#measure1"/>
                                                                                                        <swrl:argument2 rdf:resource="urn:swrl#value1"/>
                                                                                                    </rdf:Description>
                                                                                                </rdf:first>
                                                                                            </rdf:Description>
                                                                                        </rdf:rest>
                                                                                        <rdf:first>
                                                                                            <rdf:Description>
                                                                                                <rdf:type rdf:resource="&swrl;SameIndividualAtom"/>
                                                                                                <swrl:argument1 rdf:resource="urn:swrl#individual1"/>
                                                                                                <swrl:argument2 rdf:resource="urn:swrl#individual2"/>
                                                                                            </rdf:Description>
                                                                                        </rdf:first>
                                                                                    </rdf:Description>
                                                                                </rdf:rest>
                                                                            </rdf:Description>
                                                                        </rdf:rest>
                                                                    </rdf:Description>
                                                                </rdf:rest>
                                                                <rdf:first>
                                                                    <rdf:Description>
                                                                        <rdf:type rdf:resource="&swrl;IndividualPropertyAtom"/>
                                                                        <swrl:propertyPredicate rdf:resource="http://purl.org/ceu/simeon#hasTargetObject"/>
                                                                        <swrl:argument2 rdf:resource="urn:swrl#individual3"/>
                                                                        <swrl:argument1 rdf:resource="urn:swrl#measure2"/>
                                                                    </rdf:Description>
                                                                </rdf:first>
                                                            </rdf:Description>
                                                        </rdf:rest>
                                                    </rdf:Description>
                                                </rdf:rest>
                                            </rdf:Description>
                                        </rdf:rest>
                                    </rdf:Description>
                                </rdf:rest>
                                <rdf:first>
                                    <rdf:Description>
                                        <rdf:type rdf:resource="&swrl;ClassAtom"/>
                                        <swrl:classPredicate rdf:resource="http://purl.org/ceu/simeon#SimilarityMeasure"/>
                                        <swrl:argument1 rdf:resource="urn:swrl#measure1"/>
                                    </rdf:Description>
                                </rdf:first>
                            </rdf:Description>
                        </rdf:rest>
                        <rdf:first>
                            <rdf:Description>
                                <rdf:type rdf:resource="&swrl;IndividualPropertyAtom"/>
                                <swrl:propertyPredicate rdf:resource="http://purl.org/ceu/simeon#usesComparisonMethod"/>
                                <swrl:argument1 rdf:resource="urn:swrl#measure2"/>
                                <swrl:argument2 rdf:resource="urn:swrl#method"/>
                            </rdf:Description>
                        </rdf:first>
                    </rdf:Description>
                </rdf:rest>
            </rdf:Description>
        </swrl:body>
    </rdf:Description>
    <rdf:Description>
        <rdf:type rdf:resource="&swrl;Imp"/>
        <swrl:head>
            <rdf:Description>
                <rdf:type rdf:resource="&swrl;AtomList"/>
                <rdf:rest rdf:resource="&rdf;nil"/>
                <rdf:first>
                    <rdf:Description>
                        <rdf:type rdf:resource="&swrl;DatavaluedPropertyAtom"/>
                        <swrl:argument2 rdf:datatype="&xsd;integer">0</swrl:argument2>
                        <swrl:propertyPredicate rdf:resource="http://purl.org/ceu/simeon#hasValue"/>
                        <swrl:argument1 rdf:resource="urn:swrl#measure"/>
                    </rdf:Description>
                </rdf:first>
            </rdf:Description>
        </swrl:head>
        <swrl:body>
            <rdf:Description>
                <rdf:type rdf:resource="&swrl;AtomList"/>
                <rdf:first>
                    <rdf:Description>
                        <rdf:type rdf:resource="&swrl;IndividualPropertyAtom"/>
                        <swrl:propertyPredicate rdf:resource="http://purl.org/ceu/simeon#hasSourceObject"/>
                        <swrl:argument2 rdf:resource="urn:swrl#individual1"/>
                        <swrl:argument1 rdf:resource="urn:swrl#measure"/>
                    </rdf:Description>
                </rdf:first>
                <rdf:rest>
                    <rdf:Description>
                        <rdf:type rdf:resource="&swrl;AtomList"/>
                        <rdf:first>
                            <rdf:Description>
                                <rdf:type rdf:resource="&swrl;IndividualPropertyAtom"/>
                                <swrl:propertyPredicate rdf:resource="http://purl.org/ceu/simeon#hasTargetObject"/>
                                <swrl:argument2 rdf:resource="urn:swrl#individual2"/>
                                <swrl:argument1 rdf:resource="urn:swrl#measure"/>
                            </rdf:Description>
                        </rdf:first>
                        <rdf:rest>
                            <rdf:Description>
                                <rdf:type rdf:resource="&swrl;AtomList"/>
                                <rdf:rest>
                                    <rdf:Description>
                                        <rdf:type rdf:resource="&swrl;AtomList"/>
                                        <rdf:rest rdf:resource="&rdf;nil"/>
                                        <rdf:first>
                                            <rdf:Description>
                                                <rdf:type rdf:resource="&swrl;SameIndividualAtom"/>
                                                <swrl:argument1 rdf:resource="urn:swrl#individual1"/>
                                                <swrl:argument2 rdf:resource="urn:swrl#individual2"/>
                                            </rdf:Description>
                                        </rdf:first>
                                    </rdf:Description>
                                </rdf:rest>
                                <rdf:first>
                                    <rdf:Description>
                                        <rdf:type rdf:resource="&swrl;ClassAtom"/>
                                        <swrl:classPredicate rdf:resource="http://purl.org/ceu/simeon#DissimilarityMeasure"/>
                                        <swrl:argument1 rdf:resource="urn:swrl#measure"/>
                                    </rdf:Description>
                                </rdf:first>
                            </rdf:Description>
                        </rdf:rest>
                    </rdf:Description>
                </rdf:rest>
            </rdf:Description>
        </swrl:body>
    </rdf:Description>
    <rdf:Description>
        <rdf:type rdf:resource="&swrl;Imp"/>
        <swrl:head>
            <rdf:Description>
                <rdf:type rdf:resource="&swrl;AtomList"/>
                <rdf:rest rdf:resource="&rdf;nil"/>
                <rdf:first>
                    <rdf:Description>
                        <rdf:type rdf:resource="&swrl;DatavaluedPropertyAtom"/>
                        <swrl:argument2 rdf:datatype="&xsd;integer">1</swrl:argument2>
                        <swrl:propertyPredicate rdf:resource="http://purl.org/ceu/simeon#hasValue"/>
                        <swrl:argument1 rdf:resource="urn:swrl#similarity"/>
                    </rdf:Description>
                </rdf:first>
            </rdf:Description>
        </swrl:head>
        <swrl:body>
            <rdf:Description>
                <rdf:type rdf:resource="&swrl;AtomList"/>
                <rdf:first>
                    <rdf:Description>
                        <rdf:type rdf:resource="&swrl;IndividualPropertyAtom"/>
                        <swrl:propertyPredicate rdf:resource="http://purl.org/ceu/simeon#hasSourceObject"/>
                        <swrl:argument2 rdf:resource="urn:swrl#individual1"/>
                        <swrl:argument1 rdf:resource="urn:swrl#similarity"/>
                    </rdf:Description>
                </rdf:first>
                <rdf:rest>
                    <rdf:Description>
                        <rdf:type rdf:resource="&swrl;AtomList"/>
                        <rdf:rest>
                            <rdf:Description>
                                <rdf:type rdf:resource="&swrl;AtomList"/>
                                <rdf:first>
                                    <rdf:Description>
                                        <rdf:type rdf:resource="&swrl;ClassAtom"/>
                                        <swrl:classPredicate rdf:resource="http://purl.org/ceu/simeon#NormalizedSimilarityMeasure"/>
                                        <swrl:argument1 rdf:resource="urn:swrl#similarity"/>
                                    </rdf:Description>
                                </rdf:first>
                                <rdf:rest>
                                    <rdf:Description>
                                        <rdf:type rdf:resource="&swrl;AtomList"/>
                                        <rdf:rest rdf:resource="&rdf;nil"/>
                                        <rdf:first>
                                            <rdf:Description>
                                                <rdf:type rdf:resource="&swrl;SameIndividualAtom"/>
                                                <swrl:argument1 rdf:resource="urn:swrl#individual1"/>
                                                <swrl:argument2 rdf:resource="urn:swrl#individual2"/>
                                            </rdf:Description>
                                        </rdf:first>
                                    </rdf:Description>
                                </rdf:rest>
                            </rdf:Description>
                        </rdf:rest>
                        <rdf:first>
                            <rdf:Description>
                                <rdf:type rdf:resource="&swrl;IndividualPropertyAtom"/>
                                <swrl:propertyPredicate rdf:resource="http://purl.org/ceu/simeon#hasTargetObject"/>
                                <swrl:argument2 rdf:resource="urn:swrl#individual2"/>
                                <swrl:argument1 rdf:resource="urn:swrl#similarity"/>
                            </rdf:Description>
                        </rdf:first>
                    </rdf:Description>
                </rdf:rest>
            </rdf:Description>
        </swrl:body>
    </rdf:Description>
    <rdf:Description>
        <rdf:type rdf:resource="&swrl;Imp"/>
        <swrl:body>
            <rdf:Description>
                <rdf:type rdf:resource="&swrl;AtomList"/>
                <rdf:rest>
                    <rdf:Description>
                        <rdf:type rdf:resource="&swrl;AtomList"/>
                        <rdf:first>
                            <rdf:Description>
                                <rdf:type rdf:resource="&swrl;ClassAtom"/>
                                <swrl:classPredicate rdf:resource="http://purl.org/ceu/simeon#NormalizedSimilarityMeasure"/>
                                <swrl:argument1 rdf:resource="urn:swrl#similarity"/>
                            </rdf:Description>
                        </rdf:first>
                        <rdf:rest>
                            <rdf:Description>
                                <rdf:type rdf:resource="&swrl;AtomList"/>
                                <rdf:rest>
                                    <rdf:Description>
                                        <rdf:type rdf:resource="&swrl;AtomList"/>
                                        <rdf:rest rdf:resource="&rdf;nil"/>
                                        <rdf:first>
                                            <rdf:Description>
                                                <rdf:type rdf:resource="&swrl;DatavaluedPropertyAtom"/>
                                                <swrl:propertyPredicate rdf:resource="http://purl.org/ceu/simeon#hasSourceData"/>
                                                <swrl:argument2 rdf:resource="urn:swrl#literal1"/>
                                                <swrl:argument1 rdf:resource="urn:swrl#similarity"/>
                                            </rdf:Description>
                                        </rdf:first>
                                    </rdf:Description>
                                </rdf:rest>
                                <rdf:first>
                                    <rdf:Description>
                                        <rdf:type rdf:resource="&swrl;SameIndividualAtom"/>
                                        <swrl:argument1 rdf:resource="urn:swrl#literal1"/>
                                        <swrl:argument2 rdf:resource="urn:swrl#literal2"/>
                                    </rdf:Description>
                                </rdf:first>
                            </rdf:Description>
                        </rdf:rest>
                    </rdf:Description>
                </rdf:rest>
                <rdf:first>
                    <rdf:Description>
                        <rdf:type rdf:resource="&swrl;DatavaluedPropertyAtom"/>
                        <swrl:propertyPredicate rdf:resource="http://purl.org/ceu/simeon#hasTargetData"/>
                        <swrl:argument2 rdf:resource="urn:swrl#literal2"/>
                        <swrl:argument1 rdf:resource="urn:swrl#similarity"/>
                    </rdf:Description>
                </rdf:first>
            </rdf:Description>
        </swrl:body>
        <swrl:head>
            <rdf:Description>
                <rdf:type rdf:resource="&swrl;AtomList"/>
                <rdf:rest rdf:resource="&rdf;nil"/>
                <rdf:first>
                    <rdf:Description>
                        <rdf:type rdf:resource="&swrl;DatavaluedPropertyAtom"/>
                        <swrl:argument2 rdf:datatype="&xsd;integer">1</swrl:argument2>
                        <swrl:propertyPredicate rdf:resource="http://purl.org/ceu/simeon#hasValue"/>
                        <swrl:argument1 rdf:resource="urn:swrl#similarity"/>
                    </rdf:Description>
                </rdf:first>
            </rdf:Description>
        </swrl:head>
    </rdf:Description>
    <rdf:Description>
        <rdf:type rdf:resource="&swrl;Imp"/>
        <swrl:head>
            <rdf:Description>
                <rdf:type rdf:resource="&swrl;AtomList"/>
                <rdf:rest>
                    <rdf:Description>
                        <rdf:type rdf:resource="&swrl;AtomList"/>
                        <rdf:rest>
                            <rdf:Description>
                                <rdf:type rdf:resource="&swrl;AtomList"/>
                                <rdf:rest>
                                    <rdf:Description>
                                        <rdf:type rdf:resource="&swrl;AtomList"/>
                                        <rdf:rest>
                                            <rdf:Description>
                                                <rdf:type rdf:resource="&swrl;AtomList"/>
                                                <rdf:rest rdf:resource="&rdf;nil"/>
                                                <rdf:first>
                                                    <rdf:Description>
                                                        <rdf:type rdf:resource="&swrl;IndividualPropertyAtom"/>
                                                        <swrl:propertyPredicate rdf:resource="http://purl.org/ceu/simeon#hasSourceObject"/>
                                                        <swrl:argument2 rdf:resource="urn:swrl#individual2"/>
                                                        <swrl:argument1 rdf:resource="urn:swrl#measure2"/>
                                                    </rdf:Description>
                                                </rdf:first>
                                            </rdf:Description>
                                        </rdf:rest>
                                        <rdf:first>
                                            <rdf:Description>
                                                <rdf:type rdf:resource="&swrl;DatavaluedPropertyAtom"/>
                                                <swrl:propertyPredicate rdf:resource="http://purl.org/ceu/simeon#hasValue"/>
                                                <swrl:argument1 rdf:resource="urn:swrl#measure2"/>
                                                <swrl:argument2 rdf:resource="urn:swrl#value"/>
                                            </rdf:Description>
                                        </rdf:first>
                                    </rdf:Description>
                                </rdf:rest>
                                <rdf:first>
                                    <rdf:Description>
                                        <rdf:type rdf:resource="&swrl;IndividualPropertyAtom"/>
                                        <swrl:propertyPredicate rdf:resource="http://purl.org/ceu/simeon#usesComparisonMethod"/>
                                        <swrl:argument1 rdf:resource="urn:swrl#measure2"/>
                                        <swrl:argument2 rdf:resource="urn:swrl#method"/>
                                    </rdf:Description>
                                </rdf:first>
                            </rdf:Description>
                        </rdf:rest>
                        <rdf:first>
                            <rdf:Description>
                                <rdf:type rdf:resource="&swrl;IndividualPropertyAtom"/>
                                <swrl:propertyPredicate rdf:resource="http://purl.org/ceu/simeon#hasTargetObject"/>
                                <swrl:argument2 rdf:resource="urn:swrl#individual1"/>
                                <swrl:argument1 rdf:resource="urn:swrl#measure2"/>
                            </rdf:Description>
                        </rdf:first>
                    </rdf:Description>
                </rdf:rest>
                <rdf:first>
                    <rdf:Description>
                        <rdf:type rdf:resource="&swrl;ClassAtom"/>
                        <swrl:classPredicate rdf:resource="http://purl.org/ceu/simeon#SymmetricComparisonMeasure"/>
                        <swrl:argument1 rdf:resource="urn:swrl#measure2"/>
                    </rdf:Description>
                </rdf:first>
            </rdf:Description>
        </swrl:head>
        <swrl:body>
            <rdf:Description>
                <rdf:type rdf:resource="&swrl;AtomList"/>
                <rdf:rest>
                    <rdf:Description>
                        <rdf:type rdf:resource="&swrl;AtomList"/>
                        <rdf:rest>
                            <rdf:Description>
                                <rdf:type rdf:resource="&swrl;AtomList"/>
                                <rdf:rest>
                                    <rdf:Description>
                                        <rdf:type rdf:resource="&swrl;AtomList"/>
                                        <rdf:rest>
                                            <rdf:Description>
                                                <rdf:type rdf:resource="&swrl;AtomList"/>
                                                <rdf:rest rdf:resource="&rdf;nil"/>
                                                <rdf:first>
                                                    <rdf:Description>
                                                        <rdf:type rdf:resource="&swrl;IndividualPropertyAtom"/>
                                                        <swrl:propertyPredicate rdf:resource="http://purl.org/ceu/simeon#hasTargetObject"/>
                                                        <swrl:argument2 rdf:resource="urn:swrl#individual2"/>
                                                        <swrl:argument1 rdf:resource="urn:swrl#measure1"/>
                                                    </rdf:Description>
                                                </rdf:first>
                                            </rdf:Description>
                                        </rdf:rest>
                                        <rdf:first>
                                            <rdf:Description>
                                                <rdf:type rdf:resource="&swrl;IndividualPropertyAtom"/>
                                                <swrl:propertyPredicate rdf:resource="http://purl.org/ceu/simeon#hasSourceObject"/>
                                                <swrl:argument2 rdf:resource="urn:swrl#individual1"/>
                                                <swrl:argument1 rdf:resource="urn:swrl#measure1"/>
                                            </rdf:Description>
                                        </rdf:first>
                                    </rdf:Description>
                                </rdf:rest>
                                <rdf:first>
                                    <rdf:Description>
                                        <rdf:type rdf:resource="&swrl;DatavaluedPropertyAtom"/>
                                        <swrl:propertyPredicate rdf:resource="http://purl.org/ceu/simeon#hasValue"/>
                                        <swrl:argument1 rdf:resource="urn:swrl#measure1"/>
                                        <swrl:argument2 rdf:resource="urn:swrl#value"/>
                                    </rdf:Description>
                                </rdf:first>
                            </rdf:Description>
                        </rdf:rest>
                        <rdf:first>
                            <rdf:Description>
                                <rdf:type rdf:resource="&swrl;IndividualPropertyAtom"/>
                                <swrl:propertyPredicate rdf:resource="http://purl.org/ceu/simeon#usesComparisonMethod"/>
                                <swrl:argument1 rdf:resource="urn:swrl#measure1"/>
                                <swrl:argument2 rdf:resource="urn:swrl#method"/>
                            </rdf:Description>
                        </rdf:first>
                    </rdf:Description>
                </rdf:rest>
                <rdf:first>
                    <rdf:Description>
                        <rdf:type rdf:resource="&swrl;ClassAtom"/>
                        <swrl:classPredicate rdf:resource="http://purl.org/ceu/simeon#SymmetricComparisonMeasure"/>
                        <swrl:argument1 rdf:resource="urn:swrl#measure1"/>
                    </rdf:Description>
                </rdf:first>
            </rdf:Description>
        </swrl:body>
    </rdf:Description>
    <rdf:Description>
        <rdf:type rdf:resource="&swrl;Imp"/>
        <swrl:head>
            <rdf:Description>
                <rdf:type rdf:resource="&swrl;AtomList"/>
                <rdf:rest rdf:resource="&rdf;nil"/>
                <rdf:first>
                    <rdf:Description>
                        <rdf:type rdf:resource="&swrl;DatavaluedPropertyAtom"/>
                        <swrl:argument2 rdf:datatype="&xsd;integer">0</swrl:argument2>
                        <swrl:propertyPredicate rdf:resource="http://purl.org/ceu/simeon#hasValue"/>
                        <swrl:argument1 rdf:resource="urn:swrl#measure"/>
                    </rdf:Description>
                </rdf:first>
            </rdf:Description>
        </swrl:head>
        <swrl:body>
            <rdf:Description>
                <rdf:type rdf:resource="&swrl;AtomList"/>
                <rdf:first>
                    <rdf:Description>
                        <rdf:type rdf:resource="&swrl;ClassAtom"/>
                        <swrl:classPredicate rdf:resource="http://purl.org/ceu/simeon#SimilarityMeasure"/>
                        <swrl:argument1 rdf:resource="urn:swrl#measure"/>
                    </rdf:Description>
                </rdf:first>
                <rdf:rest>
                    <rdf:Description>
                        <rdf:type rdf:resource="&swrl;AtomList"/>
                        <rdf:first>
                            <rdf:Description>
                                <rdf:type rdf:resource="&swrl;DatavaluedPropertyAtom"/>
                                <swrl:propertyPredicate rdf:resource="http://purl.org/ceu/simeon#hasSourceData"/>
                                <swrl:argument2 rdf:resource="urn:swrl#literal1"/>
                                <swrl:argument1 rdf:resource="urn:swrl#measure"/>
                            </rdf:Description>
                        </rdf:first>
                        <rdf:rest>
                            <rdf:Description>
                                <rdf:type rdf:resource="&swrl;AtomList"/>
                                <rdf:rest>
                                    <rdf:Description>
                                        <rdf:type rdf:resource="&swrl;AtomList"/>
                                        <rdf:rest>
                                            <rdf:Description>
                                                <rdf:type rdf:resource="&swrl;AtomList"/>
                                                <rdf:rest rdf:resource="&rdf;nil"/>
                                                <rdf:first>
                                                    <rdf:Description>
                                                        <rdf:type rdf:resource="&swrl;DifferentIndividualsAtom"/>
                                                        <swrl:argument1 rdf:resource="urn:swrl#literal1"/>
                                                        <swrl:argument2 rdf:resource="urn:swrl#literal2"/>
                                                    </rdf:Description>
                                                </rdf:first>
                                            </rdf:Description>
                                        </rdf:rest>
                                        <rdf:first>
                                            <rdf:Description>
                                                <rdf:type rdf:resource="&swrl;IndividualPropertyAtom"/>
                                                <swrl:argument2 rdf:resource="http://purl.org/ceu/simeon#dataIdentitySimilarityFunction"/>
                                                <swrl:propertyPredicate rdf:resource="http://purl.org/ceu/simeon#usesComparisonMethod"/>
                                                <swrl:argument1 rdf:resource="urn:swrl#measure"/>
                                            </rdf:Description>
                                        </rdf:first>
                                    </rdf:Description>
                                </rdf:rest>
                                <rdf:first>
                                    <rdf:Description>
                                        <rdf:type rdf:resource="&swrl;DatavaluedPropertyAtom"/>
                                        <swrl:propertyPredicate rdf:resource="http://purl.org/ceu/simeon#hasTargetData"/>
                                        <swrl:argument2 rdf:resource="urn:swrl#literal2"/>
                                        <swrl:argument1 rdf:resource="urn:swrl#measure"/>
                                    </rdf:Description>
                                </rdf:first>
                            </rdf:Description>
                        </rdf:rest>
                    </rdf:Description>
                </rdf:rest>
            </rdf:Description>
        </swrl:body>
    </rdf:Description>
    <rdf:Description>
        <rdf:type rdf:resource="&swrl;Imp"/>
        <swrl:body>
            <rdf:Description>
                <rdf:type rdf:resource="&swrl;AtomList"/>
                <rdf:first>
                    <rdf:Description>
                        <rdf:type rdf:resource="&swrl;IndividualPropertyAtom"/>
                        <swrl:propertyPredicate rdf:resource="http://purl.org/ceu/simeon#usesComparisonMethod"/>
                        <swrl:argument1 rdf:resource="urn:swrl#measure2"/>
                        <swrl:argument2 rdf:resource="urn:swrl#method"/>
                    </rdf:Description>
                </rdf:first>
                <rdf:rest>
                    <rdf:Description>
                        <rdf:type rdf:resource="&swrl;AtomList"/>
                        <rdf:rest>
                            <rdf:Description>
                                <rdf:type rdf:resource="&swrl;AtomList"/>
                                <rdf:first>
                                    <rdf:Description>
                                        <rdf:type rdf:resource="&swrl;DatavaluedPropertyAtom"/>
                                        <swrl:propertyPredicate rdf:resource="http://purl.org/ceu/simeon#hasSourceData"/>
                                        <swrl:argument2 rdf:resource="urn:swrl#literal1"/>
                                        <swrl:argument1 rdf:resource="urn:swrl#measure1"/>
                                    </rdf:Description>
                                </rdf:first>
                                <rdf:rest>
                                    <rdf:Description>
                                        <rdf:type rdf:resource="&swrl;AtomList"/>
                                        <rdf:rest>
                                            <rdf:Description>
                                                <rdf:type rdf:resource="&swrl;AtomList"/>
                                                <rdf:first>
                                                    <rdf:Description>
                                                        <rdf:type rdf:resource="&swrl;SameIndividualAtom"/>
                                                        <swrl:argument1 rdf:resource="urn:swrl#literal1"/>
                                                        <swrl:argument2 rdf:resource="urn:swrl#literal2"/>
                                                    </rdf:Description>
                                                </rdf:first>
                                                <rdf:rest>
                                                    <rdf:Description>
                                                        <rdf:type rdf:resource="&swrl;AtomList"/>
                                                        <rdf:rest>
                                                            <rdf:Description>
                                                                <rdf:type rdf:resource="&swrl;AtomList"/>
                                                                <rdf:first>
                                                                    <rdf:Description>
                                                                        <rdf:type rdf:resource="&swrl;DatavaluedPropertyAtom"/>
                                                                        <swrl:propertyPredicate rdf:resource="http://purl.org/ceu/simeon#hasValue"/>
                                                                        <swrl:argument1 rdf:resource="urn:swrl#measure2"/>
                                                                        <swrl:argument2 rdf:resource="urn:swrl#value2"/>
                                                                    </rdf:Description>
                                                                </rdf:first>
                                                                <rdf:rest>
                                                                    <rdf:Description>
                                                                        <rdf:type rdf:resource="&swrl;AtomList"/>
                                                                        <rdf:first>
                                                                            <rdf:Description>
                                                                                <rdf:type rdf:resource="&swrl;ClassAtom"/>
                                                                                <swrl:classPredicate rdf:resource="http://purl.org/ceu/simeon#SimilarityMeasure"/>
                                                                                <swrl:argument1 rdf:resource="urn:swrl#measure2"/>
                                                                            </rdf:Description>
                                                                        </rdf:first>
                                                                        <rdf:rest>
                                                                            <rdf:Description>
                                                                                <rdf:type rdf:resource="&swrl;AtomList"/>
                                                                                <rdf:first>
                                                                                    <rdf:Description>
                                                                                        <rdf:type rdf:resource="&swrl;DatavaluedPropertyAtom"/>
                                                                                        <swrl:propertyPredicate rdf:resource="http://purl.org/ceu/simeon#hasValue"/>
                                                                                        <swrl:argument1 rdf:resource="urn:swrl#measure1"/>
                                                                                        <swrl:argument2 rdf:resource="urn:swrl#value1"/>
                                                                                    </rdf:Description>
                                                                                </rdf:first>
                                                                                <rdf:rest>
                                                                                    <rdf:Description>
                                                                                        <rdf:type rdf:resource="&swrl;AtomList"/>
                                                                                        <rdf:first>
                                                                                            <rdf:Description>
                                                                                                <rdf:type rdf:resource="&swrl;DatavaluedPropertyAtom"/>
                                                                                                <swrl:propertyPredicate rdf:resource="http://purl.org/ceu/simeon#hasSourceData"/>
                                                                                                <swrl:argument2 rdf:resource="urn:swrl#literal1"/>
                                                                                                <swrl:argument1 rdf:resource="urn:swrl#measure2"/>
                                                                                            </rdf:Description>
                                                                                        </rdf:first>
                                                                                        <rdf:rest>
                                                                                            <rdf:Description>
                                                                                                <rdf:type rdf:resource="&swrl;AtomList"/>
                                                                                                <rdf:rest rdf:resource="&rdf;nil"/>
                                                                                                <rdf:first>
                                                                                                    <rdf:Description>
                                                                                                        <rdf:type rdf:resource="&swrl;DatavaluedPropertyAtom"/>
                                                                                                        <swrl:propertyPredicate rdf:resource="http://purl.org/ceu/simeon#hasTargetData"/>
                                                                                                        <swrl:argument2 rdf:resource="urn:swrl#literal3"/>
                                                                                                        <swrl:argument1 rdf:resource="urn:swrl#measure2"/>
                                                                                                    </rdf:Description>
                                                                                                </rdf:first>
                                                                                            </rdf:Description>
                                                                                        </rdf:rest>
                                                                                    </rdf:Description>
                                                                                </rdf:rest>
                                                                            </rdf:Description>
                                                                        </rdf:rest>
                                                                    </rdf:Description>
                                                                </rdf:rest>
                                                            </rdf:Description>
                                                        </rdf:rest>
                                                        <rdf:first>
                                                            <rdf:Description>
                                                                <rdf:type rdf:resource="&swrl;IndividualPropertyAtom"/>
                                                                <swrl:propertyPredicate rdf:resource="http://purl.org/ceu/simeon#usesComparisonMethod"/>
                                                                <swrl:argument1 rdf:resource="urn:swrl#measure1"/>
                                                                <swrl:argument2 rdf:resource="urn:swrl#method"/>
                                                            </rdf:Description>
                                                        </rdf:first>
                                                    </rdf:Description>
                                                </rdf:rest>
                                            </rdf:Description>
                                        </rdf:rest>
                                        <rdf:first>
                                            <rdf:Description>
                                                <rdf:type rdf:resource="&swrl;DatavaluedPropertyAtom"/>
                                                <swrl:propertyPredicate rdf:resource="http://purl.org/ceu/simeon#hasTargetData"/>
                                                <swrl:argument2 rdf:resource="urn:swrl#literal1"/>
                                                <swrl:argument1 rdf:resource="urn:swrl#measure1"/>
                                            </rdf:Description>
                                        </rdf:first>
                                    </rdf:Description>
                                </rdf:rest>
                            </rdf:Description>
                        </rdf:rest>
                        <rdf:first>
                            <rdf:Description>
                                <rdf:type rdf:resource="&swrl;ClassAtom"/>
                                <swrl:classPredicate rdf:resource="http://purl.org/ceu/simeon#SimilarityMeasure"/>
                                <swrl:argument1 rdf:resource="urn:swrl#measure1"/>
                            </rdf:Description>
                        </rdf:first>
                    </rdf:Description>
                </rdf:rest>
            </rdf:Description>
        </swrl:body>
        <swrl:head>
            <rdf:Description>
                <rdf:type rdf:resource="&swrl;AtomList"/>
                <rdf:rest rdf:resource="&rdf;nil"/>
                <rdf:first>
                    <rdf:Description>
                        <rdf:type rdf:resource="&swrl;BuiltinAtom"/>
                        <swrl:builtin rdf:resource="&swrlb;greaterThanOrEqual"/>
                        <swrl:arguments rdf:parseType="Collection">
                            <rdf:Description rdf:about="urn:swrl#value1"/>
                            <rdf:Description rdf:about="urn:swrl#value2"/>
                        </swrl:arguments>
                    </rdf:Description>
                </rdf:first>
            </rdf:Description>
        </swrl:head>
    </rdf:Description>
</rdf:RDF>



<!-- Generated by the OWL API (version 3.5.1) http://owlapi.sourceforge.net -->

